@prefix : <http://www.semanticweb.org/patric/ontologies/2025/3/Programming_Languages_Ontology#> .
@prefix owl: <http://www.w3.org/2002/07/owl#> .
@prefix rdf: <http://www.w3.org/1999/02/22-rdf-syntax-ns#> .
@prefix xml: <http://www.w3.org/XML/1998/namespace> .
@prefix xsd: <http://www.w3.org/2001/XMLSchema#> .
@prefix rdfs: <http://www.w3.org/2000/01/rdf-schema#> .
@base <http://www.semanticweb.org/patric/ontologies/2025/3/Programming_Languages_Ontology> .

<http://www.semanticweb.org/patric/ontologies/2025/3/Programming_Languages_Ontology> rdf:type owl:Ontology ;
                                                                                      <http://purl.org/dc/elements/1.1/creator> "Alessandro Scicolone"@en ,
                                                                                                                                "Patric Reineri"@en ;
                                                                                      <http://purl.org/dc/elements/1.1/date> "2024-05-04"@en ;
                                                                                      <http://purl.org/dc/elements/1.1/description> "An ontology describing programming languages, their paradigms, features, and relationships. It captures information about language classifications (e.g., functional, object-oriented), implementation characteristics, and historical development. The ontology aims to support knowledge representation, semantic integration, and reasoning in software engineering and educational contexts."@en ;
                                                                                      <http://purl.org/dc/elements/1.1/title> "Programming Languages Ontology"@en ;
                                                                                      <http://www.ontologydesignpatterns.org/schemas/cpannotationschema.owl#coversRequirements> "What are the elements in this set?"^^xsd:string ,
                                                                                                                                                                                "What is the cardinality (size) of this set?"^^xsd:string ,
                                                                                                                                                                                "What things are contained in this collection (community, collective)? What collections this thing is member of?" ;
                                                                                      <http://www.ontologydesignpatterns.org/schemas/cpannotationschema.owl#extractedFrom> "http://swan.mindinformatics.org/ontologies/1.2/collections.owl"^^xsd:string ,
                                                                                                                                                                           "http://www.ontologydesignpatterns.org/ont/dul/DUL.owl" ;
                                                                                      <http://www.ontologydesignpatterns.org/schemas/cpannotationschema.owl#hasAuthor> "Aldo Gangemi" ,
                                                                                                                                                                       "PaoloCiccarese"^^xsd:string ;
                                                                                      <http://www.ontologydesignpatterns.org/schemas/cpannotationschema.owl#hasConsequences> "Collections and their members can be associated. Time-indexed membership cannot be represented though (you need a situation-based pattern)." ;
                                                                                      <http://www.ontologydesignpatterns.org/schemas/cpannotationschema.owl#hasIntent> "To model sets of things (elements). A Set is a collection that cannot contain duplicate elements. "^^xsd:string ,
                                                                                                                                                                       "To represent domain (not set theory) membership." ;
                                                                                      <http://www.ontologydesignpatterns.org/schemas/cpannotationschema.owl#reengineeredFrom> "http://swan.mindinformatics.org/ontologies/1.2/collections.owl"^^xsd:string ;
                                                                                      <http://www.ontologydesignpatterns.org/schemas/cpannotationschema.owl#relatedCPs> "TimeIndexedMembership" ,
                                                                                                                                                                        "http://www.ontologydesignpatterns.org/cp/owl/bag.owl"^^xsd:string ,
                                                                                                                                                                        "http://www.ontologydesignpatterns.org/cp/owl/list.owl"^^xsd:string ;
                                                                                      <http://www.ontologydesignpatterns.org/schemas/cpannotationschema.owl#scenarios> "My saxophone collection includes a Mark VI tenor, a Balanced Action alto, and a Conn Transitional bari." ;
                                                                                      :license "MIT"@en ;
                                                                                      :vann:prederredNamespaceUri "http://www.semanticweb.org/patric/ontologies/2025/3/Programming_Languages_Ontology"@en ;
                                                                                      :vann:preferredNamespacePrefix "pl"@en ;
                                                                                      rdfs:comment "A Set is a collection that cannot contain duplicate elements. A Set is expressed by linking to it directly all the members (elements), multiple identical values of members (elements) will be eliminated because by default they are treated as a set."^^xsd:string ,
                                                                                                   """The collection entity pattern. 
It is extracted from DOLCE-UltraLite by partial clone of elements.""" ;
                                                                                      rdfs:label "Programming Languages Ontology"@en ,
                                                                                                 "collection entity" ,
                                                                                                 "membership" ;
                                                                                      owl:versionInfo "1.0"@en ,
                                                                                                      "1.1 added rdfs:isDefinedBy for all named entities"^^xsd:string ,
                                                                                                      "Created by Aldo Gangemi and Valentina Presutti"^^xsd:string ,
                                                                                                      "Created with TopBraid Composer"^^xsd:string .

#################################################################
#    Annotation properties
#################################################################

###  http://purl.org/dc/elements/1.1/creator
<http://purl.org/dc/elements/1.1/creator> rdf:type owl:AnnotationProperty .


###  http://purl.org/dc/elements/1.1/date
<http://purl.org/dc/elements/1.1/date> rdf:type owl:AnnotationProperty .


###  http://purl.org/dc/elements/1.1/description
<http://purl.org/dc/elements/1.1/description> rdf:type owl:AnnotationProperty .


###  http://purl.org/dc/elements/1.1/title
<http://purl.org/dc/elements/1.1/title> rdf:type owl:AnnotationProperty .


###  http://www.ontologydesignpatterns.org/schemas/cpannotationschema.owl#coversRequirements
<http://www.ontologydesignpatterns.org/schemas/cpannotationschema.owl#coversRequirements> rdf:type owl:AnnotationProperty ;
                                                                                          rdfs:comment "This annotation property is used for exemplifying possible requirements the content pattern provides a solution for. Requirements are expressed as natural language competency questions." .


###  http://www.ontologydesignpatterns.org/schemas/cpannotationschema.owl#extractedFrom
<http://www.ontologydesignpatterns.org/schemas/cpannotationschema.owl#extractedFrom> rdf:type owl:AnnotationProperty ;
                                                                                     rdfs:comment "This annotation property should be assigned with a URI, which points to the possible reference ontology which the annotated pattern was extracted from (i.e. the reference ontology that the ontology elements have been deeply or partially cloned by). The range is not explicit in the definition of the annotation property because it would turn the ontology to OWL Full. E.g. The participation pattern is extracted from the Dolce Ultra Lite ontology, hence the value for this annotation property is http://www.ontologydesignpatterns.org/ont/dul/DUL.owl" .


###  http://www.ontologydesignpatterns.org/schemas/cpannotationschema.owl#hasAuthor
<http://www.ontologydesignpatterns.org/schemas/cpannotationschema.owl#hasAuthor> rdf:type owl:AnnotationProperty .


###  http://www.ontologydesignpatterns.org/schemas/cpannotationschema.owl#hasConsequences
<http://www.ontologydesignpatterns.org/schemas/cpannotationschema.owl#hasConsequences> rdf:type owl:AnnotationProperty ;
                                                                                       rdfs:comment "This annotation property is used for briefly describing the benefits and/or possible trade-offs when using the CP." .


###  http://www.ontologydesignpatterns.org/schemas/cpannotationschema.owl#hasIntent
<http://www.ontologydesignpatterns.org/schemas/cpannotationschema.owl#hasIntent> rdf:type owl:AnnotationProperty ;
                                                                                 rdfs:comment "This annotation property is used in order to describe the intent of the content pattern." .


###  http://www.ontologydesignpatterns.org/schemas/cpannotationschema.owl#reengineeredFrom
<http://www.ontologydesignpatterns.org/schemas/cpannotationschema.owl#reengineeredFrom> rdf:type owl:AnnotationProperty ;
                                                                                        rdfs:comment "This annotation property should be assigned with a URI, which points to the concept schema, page, or anything else from which the annotated pattern was reengineered.  If the source does not have any URI e.g., a printed book, this property value should provide information as precise as possible in order to identify the source. This property is alternative to the extractedFrom property because it is used when the pattern come from a concept schema which is not an owl ontology. For example content ontology design patterns, which are reengineered from data model patterns, rdf schemas, etc. should be annotatd with this property. E.g. The basicpersonalfoaf pattern is extracted from the rdf FOAF specification, hence the value for this annotation property is http://xmlns.com/foaf/spec/20071002.rdf" .


###  http://www.ontologydesignpatterns.org/schemas/cpannotationschema.owl#relatedCPs
<http://www.ontologydesignpatterns.org/schemas/cpannotationschema.owl#relatedCPs> rdf:type owl:AnnotationProperty ;
                                                                                  rdfs:comment "This annotation property can be used to indicate other CPs (if any) that specialize, generalize, inlcude, or are components of the CP. Furthermore, this field may indicate other CPs that are typically used in conjunction with the described one. Important similarities and differences with other patterns can be also described here." .


###  http://www.ontologydesignpatterns.org/schemas/cpannotationschema.owl#scenarios
<http://www.ontologydesignpatterns.org/schemas/cpannotationschema.owl#scenarios> rdf:type owl:AnnotationProperty ;
                                                                                 rdfs:comment "This annotation property is used for describing examples of instantiation of the Content OP. For example, for the part-of Content OP (which represents part-whole relations) a possible scenario is the sentence: \"the brain is part of the human body\". Scenarios are expressed as natural language sentences." .


###  http://www.semanticweb.org/patric/ontologies/2025/3/Programming_Languages_Ontology#license
:license rdf:type owl:AnnotationProperty .


###  http://www.semanticweb.org/patric/ontologies/2025/3/Programming_Languages_Ontology#vann:prederredNamespaceUri
:vann:prederredNamespaceUri rdf:type owl:AnnotationProperty .


###  http://www.semanticweb.org/patric/ontologies/2025/3/Programming_Languages_Ontology#vann:preferredNamespacePrefix
:vann:preferredNamespacePrefix rdf:type owl:AnnotationProperty .


###  http://www.w3.org/2004/02/skos/core#exactMatch
<http://www.w3.org/2004/02/skos/core#exactMatch> rdf:type owl:AnnotationProperty .


#################################################################
#    Datatypes
#################################################################

###  http://www.semanticweb.org/patric/ontologies/2025/3/Programming_Languages_Ontology#architectureType
:architectureType rdf:type rdfs:Datatype ;
                  rdfs:comment "Specifies the type of computer architecture, such as x86, ARM, or MIPS, that a system or execution environment is designed to support"@en ;
                  rdfs:label "architectureType"@en ;
                  owl:equivalentClass xsd:string .


###  http://www.semanticweb.org/patric/ontologies/2025/3/Programming_Languages_Ontology#compileTimeTyping
:compileTimeTyping rdf:type rdfs:Datatype ;
                   rdfs:comment "A type system where type checking is performed during the compilation process, before the program is executed."@en ;
                   rdfs:label "compileTimeTyping"@en ;
                   owl:equivalentClass [ rdf:type rdfs:Datatype ;
                                         owl:oneOf [ rdf:type rdf:List ;
                                                     rdf:first "Dynamic" ;
                                                     rdf:rest [ rdf:type rdf:List ;
                                                                rdf:first "Static" ;
                                                                rdf:rest rdf:nil
                                                              ]
                                                   ]
                                       ] .


###  http://www.semanticweb.org/patric/ontologies/2025/3/Programming_Languages_Ontology#esecutionTimeTyping
:esecutionTimeTyping rdf:type rdfs:Datatype ;
                     rdfs:comment "A type system where type checking is performed at runtime, during the execution of the program, rather than at compile time."@en ;
                     rdfs:label "esecutionTimeTyping"@en ;
                     owl:equivalentClass [ rdf:type rdfs:Datatype ;
                                           owl:oneOf [ rdf:type rdf:List ;
                                                       rdf:first "Strong" ;
                                                       rdf:rest [ rdf:type rdf:List ;
                                                                  rdf:first "Weak" ;
                                                                  rdf:rest rdf:nil
                                                                ]
                                                     ]
                                         ] .


###  internal:anonymous-constants
<internal:anonymous-constants> rdf:type rdfs:Datatype .


#################################################################
#    Object Properties
#################################################################

###  http://www.ontologydesignpatterns.org/cp/owl/collectionentity.owl#hasMember
<http://www.ontologydesignpatterns.org/cp/owl/collectionentity.owl#hasMember> rdf:type owl:ObjectProperty ;
                                                                              owl:inverseOf <http://www.ontologydesignpatterns.org/cp/owl/collectionentity.owl#isMemberOf> ;
                                                                              rdfs:domain <http://www.ontologydesignpatterns.org/cp/owl/collectionentity.owl#Collection> ;
                                                                              rdfs:range owl:Thing ;
                                                                              rdfs:comment "A relation between collections and entities, e.g. 'my collection of saxophones includes an old Adolphe Sax original alto' (i.e. my collection has member an Adolphe Sax alto)." ,
                                                                                           "The link to the members of a Set"^^xsd:string ;
                                                                              rdfs:isDefinedBy <http://www.ontologydesignpatterns.org/cp/owl/collectionentity.owl> ;
                                                                              rdfs:label "has member"@en .


###  http://www.ontologydesignpatterns.org/cp/owl/collectionentity.owl#isMemberOf
<http://www.ontologydesignpatterns.org/cp/owl/collectionentity.owl#isMemberOf> rdf:type owl:ObjectProperty ;
                                                                               rdfs:domain owl:Thing ;
                                                                               rdfs:range <http://www.ontologydesignpatterns.org/cp/owl/collectionentity.owl#Collection> ;
                                                                               rdfs:comment "inverse of has member"@en ;
                                                                               rdfs:isDefinedBy <http://www.ontologydesignpatterns.org/cp/owl/collectionentity.owl> ;
                                                                               rdfs:label "is member of"@en .


###  http://www.semanticweb.org/patric/ontologies/2025/3/Programming_Languages_Ontology#IndirecltyDerivationFrom
:IndirecltyDerivationFrom rdf:type owl:ObjectProperty ,
                                   owl:TransitiveProperty ;
                          rdfs:domain :ProgrammingLanguage ;
                          rdfs:range :ProgrammingLanguage ;
                          owl:propertyChainAxiom ( :originatesFrom
                                                   :originatesFrom
                                                 ) ;
                          rdfs:comment "Indicates that a programming language is influenced by or derived from another programming language through one or more intermediate languages."@en ;
                          rdfs:label "indirectlyDerivationFrom"@en .


###  http://www.semanticweb.org/patric/ontologies/2025/3/Programming_Languages_Ontology#allowsDevelopmentOf
:allowsDevelopmentOf rdf:type owl:ObjectProperty ,
                              owl:FunctionalProperty ;
                     rdfs:domain :DevelopmentEnvironment ;
                     rdfs:range :ProgrammingLanguageSet ;
                     rdfs:comment "Indicates that a particular development environment enables the creation or development of a set of programming languages."@en ;
                     rdfs:label "allowsDevelopmentOf"@en .


###  http://www.semanticweb.org/patric/ontologies/2025/3/Programming_Languages_Ontology#canTranslateInto
:canTranslateInto rdf:type owl:ObjectProperty ;
                  rdfs:domain :ProgrammingLanguage ;
                  rdfs:range :MachineLanguage ;
                  owl:propertyChainAxiom ( :use
                                           :translatesInto
                                         ) ;
                  rdfs:comment "Indicates that a programming language can be translated into machine language"@en ;
                  rdfs:label "canTranslateInto"@en .


###  http://www.semanticweb.org/patric/ontologies/2025/3/Programming_Languages_Ontology#contains
:contains rdf:type owl:ObjectProperty ;
          owl:inverseOf :partOf ;
          rdfs:domain [ rdf:type owl:Class ;
                        owl:unionOf ( :DevelopmentEnvironment
                                      :ExecutionEnvironment
                                    )
                      ] ;
          rdfs:range [ rdf:type owl:Class ;
                       owl:unionOf ( :Compiler
                                     :ExecutionEnvironment
                                     :Interpreter
                                   )
                     ] ;
          rdfs:comment "Indicates that a development or execution environment includes one or more components such as a compiler, an interpreter, or another execution environment."@en ;
          rdfs:label "contains"@en .


###  http://www.semanticweb.org/patric/ontologies/2025/3/Programming_Languages_Ontology#createdBy
:createdBy rdf:type owl:ObjectProperty ;
           owl:inverseOf :isCreatorOf ;
           rdf:type owl:FunctionalProperty ;
           rdfs:domain [ rdf:type owl:Class ;
                         owl:unionOf ( :DevelopmentEnvironment
                                       :ProgrammingLanguage
                                     )
                       ] ;
           rdfs:range :ProgrammingLanguageCreator ;
           rdfs:comment "Indicates that a development environment or programming language was developed or authored by an agent, such as a person, group, or organization."@en ;
           rdfs:label "createdBy"@en .


###  http://www.semanticweb.org/patric/ontologies/2025/3/Programming_Languages_Ontology#executionRowByRowFrom
:executionRowByRowFrom rdf:type owl:ObjectProperty ;
                       rdfs:domain :Interpreter ;
                       rdfs:range :ProgrammingLanguage ;
                       rdfs:comment "Indicates that an interpreter executes a programming language line by line or statement by statement, rather than compiling the entire program before execution."@en ;
                       rdfs:label "executionRowByRow"@en .


###  http://www.semanticweb.org/patric/ontologies/2025/3/Programming_Languages_Ontology#implements
:implements rdf:type owl:ObjectProperty ;
            rdfs:domain :ProgrammingLanguage ;
            rdfs:range :ProgrammingParadigm ;
            rdfs:comment "Indicates that a programming language supports or follows a specific programming paradigm, such as functional, object-oriented, or procedural."@en ;
            rdfs:label "implements"@en .


###  http://www.semanticweb.org/patric/ontologies/2025/3/Programming_Languages_Ontology#isCreatorOf
:isCreatorOf rdf:type owl:ObjectProperty ,
                      owl:InverseFunctionalProperty ;
             rdfs:domain :ProgrammingLanguageCreator ;
             rdfs:range [ rdf:type owl:Class ;
                          owl:unionOf ( :DevelopmentEnvironment
                                        :ProgrammingLanguage
                                      )
                        ] ;
             rdfs:comment "Indicates that an agent, such as a person or organization, is the creator of a development environment or programming language."@en ;
             rdfs:label "isCreatorOf"@en .


###  http://www.semanticweb.org/patric/ontologies/2025/3/Programming_Languages_Ontology#originatesFrom
:originatesFrom rdf:type owl:ObjectProperty ,
                         owl:FunctionalProperty ;
                rdfs:domain :ProgrammingLanguage ;
                rdfs:range :ProgrammingLanguage ;
                rdfs:comment "Indicates that a programming language has its roots or foundational concepts based on another programming language."@en ;
                rdfs:label "originatesFrom"@en .


###  http://www.semanticweb.org/patric/ontologies/2025/3/Programming_Languages_Ontology#partOf
:partOf rdf:type owl:ObjectProperty ;
        rdfs:domain [ rdf:type owl:Class ;
                      owl:unionOf ( :Compiler
                                    :ExecutionEnvironment
                                    :Interpreter
                                  )
                    ] ;
        rdfs:range [ rdf:type owl:Class ;
                     owl:unionOf ( :DevelopmentEnvironment
                                   :ExecutionEnvironment
                                 )
                   ] ;
        rdfs:comment "Indicates that an entity, such as a compiler, interpreter, or execution environment, is a component within a larger development or execution environment."@en ;
        rdfs:label "partOf"@en .


###  http://www.semanticweb.org/patric/ontologies/2025/3/Programming_Languages_Ontology#translatableBy
:translatableBy rdf:type owl:ObjectProperty ;
                owl:inverseOf :translatesInto ;
                rdfs:domain :MachineLanguage ;
                rdfs:range :Compiler ;
                rdfs:comment "Indicates that machine language is the output produced by a compiler translating source code written in a programming language."@en ;
                rdfs:label "translatableBy"@en .


###  http://www.semanticweb.org/patric/ontologies/2025/3/Programming_Languages_Ontology#translateFrom
:translateFrom rdf:type owl:ObjectProperty ;
               rdfs:domain :Compiler ;
               rdfs:range :ProgrammingLanguage ;
               rdfs:comment "Indicates that a compiler takes source code written in a specific programming language as input for translation."@en ;
               rdfs:label "translateFrom"@en .


###  http://www.semanticweb.org/patric/ontologies/2025/3/Programming_Languages_Ontology#translatesInto
:translatesInto rdf:type owl:ObjectProperty ;
                rdfs:domain :Compiler ;
                rdfs:range :MachineLanguage ;
                rdfs:comment "Indicates that a compiler converts source code into machine language as part of the compilation process."@en ;
                rdfs:label "translatesInto"@en .


###  http://www.semanticweb.org/patric/ontologies/2025/3/Programming_Languages_Ontology#use
:use rdf:type owl:ObjectProperty ;
     rdfs:domain :ProgrammingLanguage ;
     rdfs:range [ rdf:type owl:Class ;
                  owl:unionOf ( :Compiler
                                :Interpreter
                              )
                ] ;
     rdfs:comment "Indicates that a programming language relies on either a compiler or an interpreter to be executed or translated."@en ;
     rdfs:label "use"@en .


###  http://www.semanticweb.org/patric/ontologies/2025/3/Programming_Languages_Ontology#writeIn
:writeIn rdf:type owl:ObjectProperty ,
                  owl:FunctionalProperty ;
         rdfs:domain <http://schema.org/SoftwareApplication> ;
         rdfs:range :ProgrammingLanguageSet ;
         rdfs:comment "Indicates that a software application is developed using one or more programming languages from a specific programming language set."@en ;
         rdfs:label "writeIn"@en .


#################################################################
#    Data properties
#################################################################

###  http://www.ontologydesignpatterns.org/cp/owl/set.owl#size
<http://www.ontologydesignpatterns.org/cp/owl/set.owl#size> rdf:type owl:DatatypeProperty ;
                                                            rdfs:domain <http://www.ontologydesignpatterns.org/cp/owl/collectionentity.owl#Collection> ;
                                                            rdfs:range xsd:integer ;
                                                            rdfs:comment "size - The number of items belonging to a collection"^^xsd:string ;
                                                            rdfs:label "size"^^xsd:string .


###  http://www.semanticweb.org/patric/ontologies/2025/3/Programming_Languages_Ontology#compatibleWith
:compatibleWith rdf:type owl:DatatypeProperty ;
                rdfs:domain :Compiler ;
                rdfs:range :architectureType ;
                rdfs:comment "Specifies the type of hardware or system architecture that a compiler is compatible with, such as x86, ARM, or MIPS."@en ;
                rdfs:label "compatibleWith"@en .


###  http://www.semanticweb.org/patric/ontologies/2025/3/Programming_Languages_Ontology#executableBy
:executableBy rdf:type owl:DatatypeProperty ;
              rdfs:domain :MachineLanguage ;
              rdfs:range :architectureType ;
              rdfs:comment "Indicates the type of system architecture capable of directly executing the given machine language code."@en ;
              rdfs:label "executableBy"@en .


###  http://www.semanticweb.org/patric/ontologies/2025/3/Programming_Languages_Ontology#hasCompileTyping
:hasCompileTyping rdf:type owl:DatatypeProperty ;
                  rdfs:subPropertyOf :hasTyping ;
                  rdf:type owl:FunctionalProperty ;
                  rdfs:domain :ProgrammingLanguage ;
                  rdfs:range :compileTimeTyping ;
                  rdfs:comment "Indicates that the programming language performs type checking during the compilation process, before the code is executed."@en ;
                  rdfs:label "hasCompileTyping"@en .


###  http://www.semanticweb.org/patric/ontologies/2025/3/Programming_Languages_Ontology#hasEsecutionTyping
:hasEsecutionTyping rdf:type owl:DatatypeProperty ;
                    rdfs:subPropertyOf :hasTyping ;
                    rdf:type owl:FunctionalProperty ;
                    rdfs:domain :ProgrammingLanguage ;
                    rdfs:range :esecutionTimeTyping ;
                    rdfs:comment "Indicates that the programming language performs type checking during program execution."@en ;
                    rdfs:label "hasEsecutionTyping"@en .


###  http://www.semanticweb.org/patric/ontologies/2025/3/Programming_Languages_Ontology#hasLogo
:hasLogo rdf:type owl:DatatypeProperty ;
         rdfs:domain :ProgrammingLanguage ;
         rdfs:range xsd:string ;
         rdfs:comment "Refers to a ProgrammingLanguage Logo"@en ;
         rdfs:label "hasLogo"@en .


###  http://www.semanticweb.org/patric/ontologies/2025/3/Programming_Languages_Ontology#hasTyping
:hasTyping rdf:type owl:DatatypeProperty ;
           rdfs:domain :ProgrammingLanguage ;
           rdfs:range [ rdf:type rdfs:Datatype ;
                        owl:unionOf ( :compileTimeTyping
                                      :esecutionTimeTyping
                                    )
                      ] ;
           rdfs:comment "Specifies whether a programming language performs type checking at compile time or at execution time."@en ;
           rdfs:label "hasTyping"@en .


###  http://www.semanticweb.org/patric/ontologies/2025/3/Programming_Languages_Ontology#isDesignedTo
:isDesignedTo rdf:type owl:DatatypeProperty ;
              rdfs:domain :ExecutionEnvironment ;
              rdfs:range :architectureType ;
              rdfs:comment "Indicates the type of hardware or system architecture for which an execution environment is specifically designed or optimized"@en ;
              rdfs:label "isDesignedTo"@en .


#################################################################
#    Classes
#################################################################

###  http://schema.org/SoftwareApplication
<http://schema.org/SoftwareApplication> rdf:type owl:Class ;
                                        rdfs:comment "A software application."@en ;
                                        rdfs:label "schema:SoftwareApplication"@en .


###  http://www.ontologydesignpatterns.org/cp/owl/collectionentity.owl#Collection
<http://www.ontologydesignpatterns.org/cp/owl/collectionentity.owl#Collection> rdf:type owl:Class ;
                                                                               rdfs:comment "Any container for entities that share one or more common properties. E.g. \"stone objects\", \"the nurses\", \"the Louvre Aegyptian collection\". A collection is not a logical class: a collection is a first-order entity, while a class is a second-order one." ;
                                                                               rdfs:isDefinedBy <http://www.ontologydesignpatterns.org/cp/owl/collectionentity.owl> ;
                                                                               rdfs:label "Collection"@en .


###  http://www.ontologydesignpatterns.org/cp/owl/set.owl#Set
<http://www.ontologydesignpatterns.org/cp/owl/set.owl#Set> rdf:type owl:Class ;
                                                           rdfs:subClassOf <http://www.ontologydesignpatterns.org/cp/owl/collectionentity.owl#Collection> ;
                                                           rdfs:comment "Set - A collection that cannot contain duplicate elements."^^xsd:string ;
                                                           rdfs:label "set"^^xsd:string .


###  http://www.semanticweb.org/patric/ontologies/2025/3/Programming_Languages_Ontology#CompiledProgrammingLanguage
:CompiledProgrammingLanguage rdf:type owl:Class ;
                             owl:equivalentClass [ rdf:type owl:Restriction ;
                                                   owl:onProperty :use ;
                                                   owl:minQualifiedCardinality "1"^^xsd:nonNegativeInteger ;
                                                   owl:onClass :Compiler
                                                 ] ;
                             rdfs:subClassOf :ProgrammingLanguage ;
                             rdfs:comment "A type of programming language in which the source code is transformed into machine code through a compiler before execution."@en ;
                             rdfs:label "CompiledProgramming Language"@en .


###  http://www.semanticweb.org/patric/ontologies/2025/3/Programming_Languages_Ontology#Compiler
:Compiler rdf:type owl:Class ;
          rdfs:comment "A software tool that translates source code written in a programming language into machine code, bytecode, or another programming language."@en ;
          rdfs:label "Compiler"@en .


###  http://www.semanticweb.org/patric/ontologies/2025/3/Programming_Languages_Ontology#DeclarativeLanguage
:DeclarativeLanguage rdf:type owl:Class ;
                     owl:equivalentClass [ rdf:type owl:Restriction ;
                                           owl:onProperty :implements ;
                                           owl:hasValue :DeclarativeParadigm
                                         ] ;
                     rdfs:subClassOf :ProgrammingLanguage ;
                     rdfs:comment "A type of programming language in which the programmer specifies what the program should accomplish rather than how it should be done, focusing on logic and expressions."@en ;
                     rdfs:label "DeclarativeLanguage"@en .


###  http://www.semanticweb.org/patric/ontologies/2025/3/Programming_Languages_Ontology#DevelopmentEnvironment
:DevelopmentEnvironment rdf:type owl:Class ;
                        rdfs:comment "A set of tools and resources used to write, test, and debug software, often including a code editor, compiler, debugger, and build automation tools."@en ;
                        rdfs:label "DevelopmentEnvironment"@en .


###  http://www.semanticweb.org/patric/ontologies/2025/3/Programming_Languages_Ontology#ExecutionEnvironment
:ExecutionEnvironment rdf:type owl:Class ;
                      rdfs:comment "The context or platform in which a program runs, including the hardware, operating system, and any supporting software or virtual machines."@en ;
                      rdfs:label "ExecutionEnvironment"@en .


###  http://www.semanticweb.org/patric/ontologies/2025/3/Programming_Languages_Ontology#FunctionalLanguage
:FunctionalLanguage rdf:type owl:Class ;
                    owl:equivalentClass [ rdf:type owl:Restriction ;
                                          owl:onProperty :implements ;
                                          owl:hasValue :FunctionalParadigm
                                        ] ;
                    rdfs:subClassOf :DeclarativeLanguage ,
                                    :Multiparadigms ;
                    rdfs:comment "A programming language that treats computation as the evaluation of mathematical functions and avoids changing state or mutable data."@en ;
                    rdfs:label "FunctionalLanguage"@en .


###  http://www.semanticweb.org/patric/ontologies/2025/3/Programming_Languages_Ontology#HighLevelCompiler
:HighLevelCompiler rdf:type owl:Class ;
                   owl:equivalentClass [ rdf:type owl:Restriction ;
                                         owl:onProperty :translateFrom ;
                                         owl:someValuesFrom :HighLevelLanguage
                                       ] ;
                   rdfs:subClassOf :Compiler ;
                   rdfs:comment "A software tool that translates programs written in high-level programming languages into lower-level machine code or intermediate representations."@en ;
                   rdfs:label "HighLevelCompiler"@en .


###  http://www.semanticweb.org/patric/ontologies/2025/3/Programming_Languages_Ontology#HighLevelLanguage
:HighLevelLanguage rdf:type owl:Class ;
                   owl:equivalentClass [ owl:intersectionOf ( [ rdf:type owl:Class ;
                                                                owl:unionOf ( [ rdf:type owl:Restriction ;
                                                                                owl:onProperty :use ;
                                                                                owl:someValuesFrom :HighLevelCompiler
                                                                              ]
                                                                              [ rdf:type owl:Restriction ;
                                                                                owl:onProperty :use ;
                                                                                owl:someValuesFrom :Interpreter
                                                                              ]
                                                                            )
                                                              ]
                                                              [ rdf:type owl:Restriction ;
                                                                owl:onProperty :implements ;
                                                                owl:someValuesFrom :ProgrammingParadigm
                                                              ]
                                                            ) ;
                                         rdf:type owl:Class
                                       ] ;
                   rdfs:subClassOf :ProgrammingLanguage ;
                   rdfs:comment "A programming language that is designed to be easy for humans to read and write, abstracting away the details of the computer's hardware."@en ;
                   rdfs:label "HighLevelLanguage"@en .


###  http://www.semanticweb.org/patric/ontologies/2025/3/Programming_Languages_Ontology#HybridProgrammingLanguage
:HybridProgrammingLanguage rdf:type owl:Class ;
                           owl:equivalentClass [ owl:intersectionOf ( [ rdf:type owl:Restriction ;
                                                                        owl:onProperty :use ;
                                                                        owl:someValuesFrom :Compiler
                                                                      ]
                                                                      [ rdf:type owl:Restriction ;
                                                                        owl:onProperty :use ;
                                                                        owl:someValuesFrom :Interpreter
                                                                      ]
                                                                    ) ;
                                                 rdf:type owl:Class
                                               ] ;
                           rdfs:subClassOf :CompiledProgrammingLanguage ,
                                           :InterpretedProgrammingLanguage ,
                                           [ owl:intersectionOf ( :CompiledProgrammingLanguage
                                                                  :InterpretedProgrammingLanguage
                                                                ) ;
                                             rdf:type owl:Class
                                           ] ;
                           rdfs:comment "A programming language that combines both compilation and interpretation, where some parts of the code are compiled and others are interpreted during execution."@en ;
                           rdfs:label "HybridProgrammingLanguage"@en .


###  http://www.semanticweb.org/patric/ontologies/2025/3/Programming_Languages_Ontology#ImperativeLanguage
:ImperativeLanguage rdf:type owl:Class ;
                    owl:equivalentClass [ rdf:type owl:Restriction ;
                                          owl:onProperty :implements ;
                                          owl:hasValue :ImperativeParadigm
                                        ] ;
                    rdfs:subClassOf :ProgrammingLanguage ;
                    rdfs:comment "A programming language that expresses the logic of a computation in terms of a sequence of statements that change the program's state."@en ;
                    rdfs:label "ImperativeLanguage"@en .


###  http://www.semanticweb.org/patric/ontologies/2025/3/Programming_Languages_Ontology#InterpretedProgrammingLanguage
:InterpretedProgrammingLanguage rdf:type owl:Class ;
                                owl:equivalentClass [ rdf:type owl:Restriction ;
                                                      owl:onProperty :use ;
                                                      owl:minQualifiedCardinality "1"^^xsd:nonNegativeInteger ;
                                                      owl:onClass :Interpreter
                                                    ] ;
                                rdfs:subClassOf :ProgrammingLanguage ;
                                rdfs:comment "A programming language in which most of the instructions are directly executed by an interpreter, without prior compilation into machine code."@en ;
                                rdfs:label "InterpretedProgrammingLanguage"@en .


###  http://www.semanticweb.org/patric/ontologies/2025/3/Programming_Languages_Ontology#Interpreter
:Interpreter rdf:type owl:Class ;
             rdfs:comment "A program that directly executes instructions written in a programming language without requiring them to be compiled into machine code."@en ;
             rdfs:label "Interpreter"@en .


###  http://www.semanticweb.org/patric/ontologies/2025/3/Programming_Languages_Ontology#LogicLanguage
:LogicLanguage rdf:type owl:Class ;
               owl:equivalentClass [ rdf:type owl:Restriction ;
                                     owl:onProperty :implements ;
                                     owl:hasValue :LogicParadigm
                                   ] ;
               rdfs:subClassOf :DeclarativeLanguage ,
                               :Multiparadigms ;
               rdfs:comment "A programming language based on formal logic, where programs are written as sets of logical statements and computation is performed through logical inference."@en ;
               rdfs:label "LogicLanguage"@en .


###  http://www.semanticweb.org/patric/ontologies/2025/3/Programming_Languages_Ontology#LowLevelCompiler
:LowLevelCompiler rdf:type owl:Class ;
                  rdfs:subClassOf :Compiler ;
                  rdfs:comment "A compiler that translates code from low-level programming languages or assembly into machine code, closely interacting with the hardware architecture."@en ;
                  rdfs:label "LowLevelCompiler"@en .


###  http://www.semanticweb.org/patric/ontologies/2025/3/Programming_Languages_Ontology#LowLevelLanguage
:LowLevelLanguage rdf:type owl:Class ;
                  rdfs:subClassOf :ProgrammingLanguage ;
                  rdfs:comment "A programming language that provides little or no abstraction from a computer's instruction set architecture, often including assembly language or machine code."@en ;
                  rdfs:label "LowLevelLanguage"@en .


###  http://www.semanticweb.org/patric/ontologies/2025/3/Programming_Languages_Ontology#MachineLanguage
:MachineLanguage rdf:type owl:Class ;
                 rdfs:subClassOf :LowLevelLanguage ;
                 rdfs:comment "A low-level programming language consisting of binary code that is directly understood and executed by a computer's central processing unit (CPU)."@en ;
                 rdfs:label "MachineLanguage"@en .


###  http://www.semanticweb.org/patric/ontologies/2025/3/Programming_Languages_Ontology#Multiparadigms
:Multiparadigms rdf:type owl:Class ;
                owl:equivalentClass [ rdf:type owl:Restriction ;
                                      owl:onProperty :implements ;
                                      owl:minQualifiedCardinality "2"^^xsd:nonNegativeInteger ;
                                      owl:onClass :ProgrammingParadigm
                                    ] ;
                rdfs:subClassOf :ProgrammingLanguage ;
                rdfs:comment "A programming language that supports multiple programming paradigms, allowing the programmer to use different styles or approaches (e.g., imperative, object-oriented, functional) within the same language."@en ;
                rdfs:label "Multiparadigms"@en .


###  http://www.semanticweb.org/patric/ontologies/2025/3/Programming_Languages_Ontology#ObjectOrientedLanguage
:ObjectOrientedLanguage rdf:type owl:Class ;
                        owl:equivalentClass [ rdf:type owl:Restriction ;
                                              owl:onProperty :implements ;
                                              owl:hasValue :ObjectOrientedParadigm
                                            ] ;
                        rdfs:subClassOf :ImperativeLanguage ,
                                        :Multiparadigms ;
                        rdfs:comment "A programming language that is based on the concept of 'objects,' which are instances of classes, and uses techniques such as inheritance, polymorphism, and encapsulation to structure software."@en ;
                        rdfs:label "Object-Oriented Language"@en .


###  http://www.semanticweb.org/patric/ontologies/2025/3/Programming_Languages_Ontology#ProceduralLanguage
:ProceduralLanguage rdf:type owl:Class ;
                    owl:equivalentClass [ rdf:type owl:Restriction ;
                                          owl:onProperty :implements ;
                                          owl:hasValue :ProceduralParadigm
                                        ] ;
                    rdfs:subClassOf :ImperativeLanguage ,
                                    :Multiparadigms ;
                    rdfs:comment "A programming language that follows a set of steps or procedures to execute a task, focusing on the sequence of actions to be performed."@en ;
                    rdfs:label "ProceduralLanguage"@en .


###  http://www.semanticweb.org/patric/ontologies/2025/3/Programming_Languages_Ontology#ProgrammingLanguage
:ProgrammingLanguage rdf:type owl:Class ;
                     owl:disjointUnionOf ( :HighLevelLanguage
                                           :LowLevelLanguage
                                         ) ;
                     rdfs:comment "A formal language comprising a set of instructions used to produce various kinds of output, primarily for creating software applications."@en ;
                     rdfs:label "ProgrammingLanguage"@en ;
                     <http://www.w3.org/2004/02/skos/core#exactMatch> <http://schema.org/ComputerLanguage> .


###  http://www.semanticweb.org/patric/ontologies/2025/3/Programming_Languages_Ontology#ProgrammingLanguageCreator
:ProgrammingLanguageCreator rdf:type owl:Class ;
                            rdfs:subClassOf <http://xmlns.com/foaf/0.1/Agent> ;
                            rdfs:comment "An individual or group responsible for designing, developing, and maintaining a programming language."@en ;
                            rdfs:label "ProgrammingLanguageCreator"@en .


###  http://www.semanticweb.org/patric/ontologies/2025/3/Programming_Languages_Ontology#ProgrammingLanguageSet
:ProgrammingLanguageSet rdf:type owl:Class ;
                        rdfs:subClassOf <http://www.ontologydesignpatterns.org/cp/owl/set.owl#Set> ;
                        rdfs:comment "A collection or group of programming languages, often categorized by purpose, paradigm, or domain of use"@en ;
                        rdfs:label "ProgrammingLanguageSet"@en .


###  http://www.semanticweb.org/patric/ontologies/2025/3/Programming_Languages_Ontology#ProgrammingParadigm
:ProgrammingParadigm rdf:type owl:Class ;
                     owl:equivalentClass [ rdf:type owl:Class ;
                                           owl:oneOf ( :DeclarativeParadigm
                                                       :EventOrientedParadigm
                                                       :FunctionalParadigm
                                                       :ImperativeParadigm
                                                       :LogicParadigm
                                                       :ObjectOrientedParadigm
                                                       :ProceduralParadigm
                                                       :StructuralParadigm
                                                     )
                                         ] ;
                     rdfs:comment "A style or approach to programming that influences how solutions are designed and implemented."@en ;
                     rdfs:label "ProgrammingParadigm"@en .


###  http://www.semanticweb.org/patric/ontologies/2025/3/Programming_Languages_Ontology#SemiCompiledProgrammingLanguage
:SemiCompiledProgrammingLanguage rdf:type owl:Class ;
                                 rdfs:subClassOf :HybridProgrammingLanguage ;
                                 rdfs:comment "A programming language that is first compiled into an intermediate code (such as bytecode) and then interpreted or executed by a runtime environment."@en ;
                                 rdfs:label "Semi-compiledProgrammingLanguage"@en .


###  http://www.semanticweb.org/patric/ontologies/2025/3/Programming_Languages_Ontology#StructuralLanguage
:StructuralLanguage rdf:type owl:Class ;
                    owl:equivalentClass [ rdf:type owl:Restriction ;
                                          owl:onProperty :implements ;
                                          owl:hasValue :StructuralParadigm
                                        ] ;
                    rdfs:subClassOf :ImperativeLanguage ,
                                    :Multiparadigms ;
                    rdfs:comment "A programming language that emphasizes the logical structure of a program, typically by organizing code into modules or blocks to improve readability and maintainability."@en ;
                    rdfs:label "StructuralLanguage"@en .


###  http://xmlns.com/foaf/0.1/Agent
<http://xmlns.com/foaf/0.1/Agent> rdf:type owl:Class ;
                                  rdfs:comment "An agent (eg. person, group, software or physical artifact)."@en ;
                                  rdfs:label "foaf:Agent"@en .


#################################################################
#    Individuals
#################################################################

###  http://www.semanticweb.org/patric/ontologies/2025/3/Programming_Languages_Ontology#ABC
:ABC rdf:type owl:NamedIndividual ,
              :HighLevelLanguage ,
              :ImperativeLanguage ,
              :InterpretedProgrammingLanguage ,
              :Multiparadigms ,
              :ProceduralLanguage ,
              :ProgrammingLanguage ;
     :implements :ImperativeParadigm ,
                 :ProceduralParadigm ;
     :use :ABCInterpreter ;
     :hasCompileTyping "Dynamic"^^:compileTimeTyping ,
                       "Dynamic"^^<internal:anonymous-constants> ;
     :hasEsecutionTyping "Strong"^^:esecutionTimeTyping ,
                         "Strong"^^<internal:anonymous-constants> ;
     :hasTyping "Dynamic"^^<internal:anonymous-constants> ,
                "Strong"^^<internal:anonymous-constants> ;
     rdfs:comment "ABC is a high-level, interactive, and interpreted programming language developed at the Centrum Wiskunde & Informatica (CWI) in the Netherlands during the 1980s. It was designed for teaching and prototyping, with an emphasis on simplicity and readability."@en ;
     rdfs:label "ABC"@en .


###  http://www.semanticweb.org/patric/ontologies/2025/3/Programming_Languages_Ontology#ABCInterpreter
:ABCInterpreter rdf:type owl:NamedIndividual ,
                         :Interpreter ;
                :executionRowByRowFrom :ABC ;
                rdfs:comment "Interpreter for ABC"@en ;
                rdfs:label "ABCInterpreter"@en .


###  http://www.semanticweb.org/patric/ontologies/2025/3/Programming_Languages_Ontology#Alan_Cooper
:Alan_Cooper rdf:type owl:NamedIndividual ,
                      :ProgrammingLanguageCreator ,
                      <http://xmlns.com/foaf/0.1/Agent> ;
             :isCreatorOf :Visual_Basic ;
             rdfs:comment "Creator of Programming Language"@en ;
             rdfs:label "Alan Cooper"@en .


###  http://www.semanticweb.org/patric/ontologies/2025/3/Programming_Languages_Ontology#Anders_Hejlsberg
:Anders_Hejlsberg rdf:type owl:NamedIndividual ,
                           :ProgrammingLanguageCreator ,
                           <http://xmlns.com/foaf/0.1/Agent> ;
                  :isCreatorOf :TypeScript ;
                  rdfs:comment "Creator of Programming Language"@en ;
                  rdfs:label "Anders Hejlsberg"@en .


###  http://www.semanticweb.org/patric/ontologies/2025/3/Programming_Languages_Ontology#Ary_Borenszweig
:Ary_Borenszweig rdf:type owl:NamedIndividual ,
                          :ProgrammingLanguageCreator ,
                          <http://xmlns.com/foaf/0.1/Agent> ;
                 :isCreatorOf :Crystal ;
                 rdfs:comment "Creator of Programming Language"@en ;
                 rdfs:label "Ary Borenszweig"@en .


###  http://www.semanticweb.org/patric/ontologies/2025/3/Programming_Languages_Ontology#Assembler
:Assembler rdf:type owl:NamedIndividual ,
                    :Compiler ,
                    :LowLevelCompiler ;
           :translateFrom :Assembly ;
           rdfs:comment "Assembly is a low-level programming language that provides a symbolic representation of a computer's machine instructions. It is architecture-specific and closely reflects the instruction set of the target CPU."@en ;
           rdfs:label "Assembler"@en .


###  http://www.semanticweb.org/patric/ontologies/2025/3/Programming_Languages_Ontology#Assembly
:Assembly rdf:type owl:NamedIndividual ,
                   :CompiledProgrammingLanguage ,
                   :ImperativeLanguage ,
                   :LowLevelLanguage ,
                   :ProgrammingLanguage ;
          :implements :ImperativeParadigm ;
          :use :Assembler ;
          rdfs:comment "Assembly is a low-level programming language that provides a symbolic representation of a computer's machine code."@en ;
          rdfs:label "Assembly"@en .


###  http://www.semanticweb.org/patric/ontologies/2025/3/Programming_Languages_Ontology#BEAM_VM
:BEAM_VM rdf:type owl:NamedIndividual ,
                  :Interpreter ;
         :executionRowByRowFrom :Erlang ;
         rdfs:comment "Interpreter of some Programming Language"@en ;
         rdfs:label "BEAM VM"@en .


###  http://www.semanticweb.org/patric/ontologies/2025/3/Programming_Languages_Ontology#Bjarne_Stroustrup
:Bjarne_Stroustrup rdf:type owl:NamedIndividual ,
                            :ProgrammingLanguageCreator ,
                            <http://xmlns.com/foaf/0.1/Agent> ;
                   :isCreatorOf <http://www.semanticweb.org/patric/ontologies/2025/3/Programming_Languages_Ontology#C++> ;
                   rdfs:comment "Creator of Programming Language"@en ;
                   rdfs:label "Bjarne Stroustrup"@en .


###  http://www.semanticweb.org/patric/ontologies/2025/3/Programming_Languages_Ontology#BrendanEich
:BrendanEich rdf:type owl:NamedIndividual ,
                      :ProgrammingLanguageCreator ,
                      <http://xmlns.com/foaf/0.1/Agent> ;
             :isCreatorOf :ECMAScript ;
             rdfs:comment "Creator of some Programming Language"@en ;
             rdfs:label "Brendan Eich"@en .


###  http://www.semanticweb.org/patric/ontologies/2025/3/Programming_Languages_Ontology#C
:C rdf:type owl:NamedIndividual ,
            :CompiledProgrammingLanguage ,
            :HighLevelLanguage ,
            :ImperativeLanguage ,
            :Multiparadigms ,
            :ProceduralLanguage ,
            :ProgrammingLanguage ,
            :StructuralLanguage ;
   <http://www.ontologydesignpatterns.org/cp/owl/collectionentity.owl#isMemberOf> :MicrosoftWordLanguageSet ,
                                                                                  :VSCodeLanguageSet ;
   :canTranslateInto :x86MachineCode ;
   :createdBy :Dennis_Ritchie ;
   :implements :ImperativeParadigm ,
               :ProceduralParadigm ,
               :StructuralParadigm ;
   :use :GCC ;
   :hasCompileTyping "Static" ;
   :hasEsecutionTyping "Strong" ;
   :hasLogo "http://commons.wikimedia.org/wiki/Special:FilePath/The%20C%20Programming%20Language%20logo.svg" ;
   :hasTyping "Static" ,
              "Strong" ;
   rdfs:comment "A low-level, general-purpose programming language that has influenced many modern languages and is widely used for system programming."@en ;
   rdfs:label "C"@en .


###  http://www.semanticweb.org/patric/ontologies/2025/3/Programming_Languages_Ontology#CPython
:CPython rdf:type owl:NamedIndividual ,
                  :Interpreter ;
         :executionRowByRowFrom :Python ;
         rdfs:comment "CPython"@en ,
                      "Python Interpreter"@en .


###  http://www.semanticweb.org/patric/ontologies/2025/3/Programming_Languages_Ontology#Chris_Lattner
:Chris_Lattner rdf:type owl:NamedIndividual ,
                        :ProgrammingLanguageCreator ,
                        <http://xmlns.com/foaf/0.1/Agent> ;
               :isCreatorOf :Swift ,
                            :SwiftUI ;
               rdfs:comment "Creator of Programming Language"@en ;
               rdfs:label "Chris Lattner"@en .


###  http://www.semanticweb.org/patric/ontologies/2025/3/Programming_Languages_Ontology#Crystal
:Crystal rdf:type owl:NamedIndividual ,
                  :CompiledProgrammingLanguage ,
                  :DeclarativeLanguage ,
                  :FunctionalLanguage ,
                  :HighLevelLanguage ,
                  :ImperativeLanguage ,
                  :Multiparadigms ,
                  :ObjectOrientedLanguage ,
                  :ProgrammingLanguage ;
         :canTranslateInto :x86MachineCode ;
         :createdBy :Ary_Borenszweig ;
         :implements :DeclarativeParadigm ,
                     :FunctionalParadigm ,
                     :ImperativeParadigm ,
                     :ObjectOrientedParadigm ;
         :originatesFrom :C ;
         :use :CrystalC ;
         :hasCompileTyping "Static" ;
         :hasEsecutionTyping "Strong" ;
         :hasLogo "http://commons.wikimedia.org/wiki/Special:FilePath/Crystal%20logo.svg" ;
         :hasTyping "Static" ,
                    "Strong" ;
         rdfs:comment "A programming language that aims to combine the performance of C with the syntax of Ruby, designed for efficiency and concurrency."@en ;
         rdfs:label "Crystal"@en .


###  http://www.semanticweb.org/patric/ontologies/2025/3/Programming_Languages_Ontology#CrystalC
:CrystalC rdf:type owl:NamedIndividual ,
                   :Compiler ,
                   :HighLevelCompiler ;
          :translateFrom :Crystal ;
          :translatesInto :x86MachineCode ;
          :compatibleWith "cross-platform"^^:architectureType ,
                          "cross-platform"^^<internal:anonymous-constants> ;
          rdfs:comment "compiler for the Crystal programming language"@en ;
          rdfs:label "CrystalC"@en .


###  http://www.semanticweb.org/patric/ontologies/2025/3/Programming_Languages_Ontology#Database_Engine
:Database_Engine rdf:type owl:NamedIndividual ,
                          :Interpreter ;
                 :executionRowByRowFrom :SQL ;
                 rdfs:comment "Interpreter of some Programming Language"@en ;
                 rdfs:label "Database Engine"@en .


###  http://www.semanticweb.org/patric/ontologies/2025/3/Programming_Languages_Ontology#DeclarativeParadigm
:DeclarativeParadigm rdf:type owl:NamedIndividual ,
                              :ProgrammingParadigm ;
                     rdfs:comment "A programming paradigm that expresses the logic of computation without describing its control flow, focusing on what to solve rather than how to solve it."@en ;
                     rdfs:label "DeclarativeParadigm"@en .


###  http://www.semanticweb.org/patric/ontologies/2025/3/Programming_Languages_Ontology#Dennis_Ritchie
:Dennis_Ritchie rdf:type owl:NamedIndividual ,
                         :ProgrammingLanguageCreator ,
                         <http://xmlns.com/foaf/0.1/Agent> ;
                :isCreatorOf :C ;
                rdfs:comment "Creator of Programming Language"@en ;
                rdfs:label "Dennis Ritchie"@en .


###  http://www.semanticweb.org/patric/ontologies/2025/3/Programming_Languages_Ontology#Donald_D._Chamberlin
:Donald_D._Chamberlin rdf:type owl:NamedIndividual ,
                               :ProgrammingLanguageCreator ,
                               <http://xmlns.com/foaf/0.1/Agent> ;
                      :isCreatorOf :SQL ;
                      rdfs:comment "Creator of Programming Language"@en ;
                      rdfs:label "Donald D. Chamberlin"@en .


###  http://www.semanticweb.org/patric/ontologies/2025/3/Programming_Languages_Ontology#Dr._Sarah_Nilsson
:Dr._Sarah_Nilsson rdf:type owl:NamedIndividual ;
                   rdfs:comment "Creator of Programming Language"@en ;
                   rdfs:label "Dr. Sarah Nilsson"@en .


###  http://www.semanticweb.org/patric/ontologies/2025/3/Programming_Languages_Ontology#ECMAScript
:ECMAScript rdf:type owl:NamedIndividual ,
                     :HighLevelLanguage ,
                     :ImperativeLanguage ,
                     :InterpretedProgrammingLanguage ,
                     :Multiparadigms ,
                     :ObjectOrientedLanguage ,
                     :ProceduralLanguage ,
                     :ProgrammingLanguage ;
            :createdBy :BrendanEich ;
            :implements :EventOrientedParadigm ,
                        :ImperativeParadigm ,
                        :ObjectOrientedParadigm ,
                        :ProceduralParadigm ;
            :use :V8 ;
            :hasCompileTyping "Dynamic"^^:esecutionTimeTyping ,
                              "Dynamic"^^<internal:anonymous-constants> ;
            :hasEsecutionTyping "Weak"^^:esecutionTimeTyping ,
                                "Weak"^^<internal:anonymous-constants> ;
            :hasTyping "Dynamic"^^<internal:anonymous-constants> ,
                       "Weak"^^<internal:anonymous-constants> .


###  http://www.semanticweb.org/patric/ontologies/2025/3/Programming_Languages_Ontology#Elixir
:Elixir rdf:type owl:NamedIndividual ,
                 :CompiledProgrammingLanguage ,
                 :DeclarativeLanguage ,
                 :FunctionalLanguage ,
                 :HighLevelLanguage ,
                 :HybridProgrammingLanguage ,
                 :InterpretedProgrammingLanguage ,
                 :Multiparadigms ,
                 :ProgrammingLanguage ,
                 :SemiCompiledProgrammingLanguage ;
        :createdBy :José_Valim ;
        :implements :DeclarativeParadigm ,
                    :EventOrientedParadigm ,
                    :FunctionalParadigm ;
        :originatesFrom :Erlang ;
        :use :BEAM_VM ,
             :ElixirC ;
        :hasCompileTyping "Dynamic" ;
        :hasEsecutionTyping "Strong" ;
        :hasLogo "http://commons.wikimedia.org/wiki/Special:FilePath/Elixir%20logo.svg" ;
        :hasTyping "Dynamic" ,
                   "Strong" ;
        rdfs:comment "A functional, concurrent language built on the Erlang VM, known for its scalability and maintainability."@en ;
        rdfs:label "Elixir"@en .


###  http://www.semanticweb.org/patric/ontologies/2025/3/Programming_Languages_Ontology#ElixirC
:ElixirC rdf:type owl:NamedIndividual ,
                  :Compiler ,
                  :HighLevelCompiler ;
         :translateFrom :Elixir ;
         rdfs:comment "compiler for the Elixir programming language"@en ;
         rdfs:label "ElixirC"@en .


###  http://www.semanticweb.org/patric/ontologies/2025/3/Programming_Languages_Ontology#Erlang
:Erlang rdf:type owl:NamedIndividual ,
                 :DeclarativeLanguage ,
                 :FunctionalLanguage ,
                 :HighLevelLanguage ,
                 :InterpretedProgrammingLanguage ,
                 :Multiparadigms ,
                 :ProgrammingLanguage ;
        :implements :DeclarativeParadigm ,
                    :FunctionalParadigm ;
        :use :BEAM_VM ;
        rdfs:comment "Erlang Programming Language"@en ;
        rdfs:label "Erlang"@en .


###  http://www.semanticweb.org/patric/ontologies/2025/3/Programming_Languages_Ontology#EventOrientedParadigm
:EventOrientedParadigm rdf:type owl:NamedIndividual ,
                                :ProgrammingParadigm ;
                       rdfs:comment "A programming paradigm where the flow of the program is determined by events such as user actions, sensor outputs."@en ;
                       rdfs:label "EventOrientedParadigm"@en .


###  http://www.semanticweb.org/patric/ontologies/2025/3/Programming_Languages_Ontology#FunctionalParadigm
:FunctionalParadigm rdf:type owl:NamedIndividual ,
                             :ProgrammingParadigm ;
                    rdfs:comment "A programming paradigm that treats computation as the evaluation of mathematical functions and avoids changing state or mutable data."@en ;
                    rdfs:label "FunctionalParadigm"@en .


###  http://www.semanticweb.org/patric/ontologies/2025/3/Programming_Languages_Ontology#GCC
:GCC rdf:type owl:NamedIndividual ,
              :Compiler ,
              :HighLevelCompiler ;
     :translateFrom :C ,
                    :GoLang ,
                    <http://www.semanticweb.org/patric/ontologies/2025/3/Programming_Languages_Ontology#C++> ;
     :translatesInto :x86MachineCode ;
     :compatibleWith "cross-platform"^^:architectureType ,
                     "cross-platform"^^<internal:anonymous-constants> ;
     rdfs:comment "optimizing compiler produced by the GNU Project, key component of the GNU tool-chain and standard compiler for most projects related to GNU and the Linux kernel."@en ;
     rdfs:label "GCC"@en .


###  http://www.semanticweb.org/patric/ontologies/2025/3/Programming_Languages_Ontology#GoLang
:GoLang rdf:type owl:NamedIndividual ,
                 :CompiledProgrammingLanguage ,
                 :HighLevelLanguage ,
                 :ImperativeLanguage ,
                 :Multiparadigms ,
                 :ProceduralLanguage ,
                 :ProgrammingLanguage ;
        <http://www.ontologydesignpatterns.org/cp/owl/collectionentity.owl#isMemberOf> :KubernetesLanguageSet ;
        :canTranslateInto :x86MachineCode ;
        :createdBy :Robert_Griesemer ;
        :implements :ImperativeParadigm ,
                    :ProceduralParadigm ;
        :originatesFrom :C ;
        :use :GCC ;
        :hasCompileTyping "Static" ;
        :hasEsecutionTyping "Strong" ;
        :hasLogo "http://commons.wikimedia.org/wiki/Special:FilePath/Go%20logo%20blue.svg" ;
        :hasTyping "Static" ,
                   "Strong" ;
        rdfs:comment "A statically typed, compiled language designed for simplicity and efficiency in system programming and web services."@en ;
        rdfs:label "GoLang"@en .


###  http://www.semanticweb.org/patric/ontologies/2025/3/Programming_Languages_Ontology#Graydon_Hoare
:Graydon_Hoare rdf:type owl:NamedIndividual ,
                        :ProgrammingLanguageCreator ,
                        <http://xmlns.com/foaf/0.1/Agent> ;
               :isCreatorOf :Rust ;
               rdfs:comment "Creator of Programming Language"@en ;
               rdfs:label "Graydon Hoare"@en .


###  http://www.semanticweb.org/patric/ontologies/2025/3/Programming_Languages_Ontology#Guido_van_Rossum
:Guido_van_Rossum rdf:type owl:NamedIndividual ,
                           :ProgrammingLanguageCreator ,
                           <http://xmlns.com/foaf/0.1/Agent> ;
                  :isCreatorOf :Python ;
                  rdfs:comment "Creator of Programming Language"@en ;
                  rdfs:label "Guido van Rossum"@en .


###  http://www.semanticweb.org/patric/ontologies/2025/3/Programming_Languages_Ontology#ImperativeParadigm
:ImperativeParadigm rdf:type owl:NamedIndividual ,
                             :ProgrammingParadigm ;
                    rdfs:comment "A programming paradigm that uses statements to change a program's state through explicit commands and control flow."@en ;
                    rdfs:label "ImperativeParadigm"@en .


###  http://www.semanticweb.org/patric/ontologies/2025/3/Programming_Languages_Ontology#IntellijIDEA
:IntellijIDEA rdf:type owl:NamedIndividual ,
                       :DevelopmentEnvironment ;
              :allowsDevelopmentOf :IntellijLanguageSet ;
              rdfs:comment "A powerful integrated development environment (IDE) primarily used for Java development, known for its intelligent code completion, debugging, and refactoring features."@en ;
              rdfs:label "IntellijIDEA"@en .


###  http://www.semanticweb.org/patric/ontologies/2025/3/Programming_Languages_Ontology#IntellijLanguageSet
:IntellijLanguageSet rdf:type owl:NamedIndividual ,
                              <http://www.ontologydesignpatterns.org/cp/owl/collectionentity.owl#Collection> ,
                              <http://www.ontologydesignpatterns.org/cp/owl/set.owl#Set> ,
                              :ProgrammingLanguageSet ;
                     <http://www.ontologydesignpatterns.org/cp/owl/collectionentity.owl#hasMember> :Java ,
                                                                                                   :Kotlin ;
                     rdfs:comment "Programming Language's Set supported by Intellij"@en ;
                     rdfs:label "IntellijLanguageSet"@en .


###  http://www.semanticweb.org/patric/ontologies/2025/3/Programming_Languages_Ontology#JRE
:JRE rdf:type owl:NamedIndividual ,
              :ExecutionEnvironment ;
     :contains :JVM ,
               :Javac ;
     rdfs:comment "JavaRuntimeEnvironment"@en ,
                  "The Java Runtime Environment (JRE) provides the libraries, Java Virtual Machine (JVM), and other components necessary to run applications written in the Java programming language. It does not include development tools such as compilers or debuggers."@en .


###  http://www.semanticweb.org/patric/ontologies/2025/3/Programming_Languages_Ontology#JVM
:JVM rdf:type owl:NamedIndividual ,
              :Interpreter ;
     :executionRowByRowFrom :Java ;
     :partOf :JRE ;
     rdfs:comment "Interpreter of some Programming Language"@en ,
                  "runtime environment that can execute Java bytecode as a result of compiling computer programs written in the Java programming language"@en ;
     rdfs:label "JVM"@en .


###  http://www.semanticweb.org/patric/ontologies/2025/3/Programming_Languages_Ontology#James_Gosling
:James_Gosling rdf:type owl:NamedIndividual ,
                        :ProgrammingLanguageCreator ,
                        <http://xmlns.com/foaf/0.1/Agent> ;
               :isCreatorOf :Java ;
               rdfs:comment "Creator of Programming Language"@en ;
               rdfs:label "James_Gosling"@en .


###  http://www.semanticweb.org/patric/ontologies/2025/3/Programming_Languages_Ontology#Java
:Java rdf:type owl:NamedIndividual ,
               :CompiledProgrammingLanguage ,
               :HighLevelLanguage ,
               :HybridProgrammingLanguage ,
               :ImperativeLanguage ,
               :InterpretedProgrammingLanguage ,
               :Multiparadigms ,
               :ObjectOrientedLanguage ,
               :ProgrammingLanguage ,
               :SemiCompiledProgrammingLanguage ;
      <http://www.ontologydesignpatterns.org/cp/owl/collectionentity.owl#isMemberOf> :IntellijLanguageSet ,
                                                                                     :MongoDBLanguageSet ,
                                                                                     :ProtègèLanguageSet ,
                                                                                     :VSCodeLanguageSet ;
      :IndirecltyDerivationFrom :C ;
      :createdBy :James_Gosling ;
      :implements :ImperativeParadigm ,
                  :ObjectOrientedParadigm ;
      :originatesFrom <http://www.semanticweb.org/patric/ontologies/2025/3/Programming_Languages_Ontology#C++> ;
      :use :JVM ,
           :Javac ;
      :hasCompileTyping "Static"^^:compileTimeTyping ,
                        "Static"^^<internal:anonymous-constants> ;
      :hasEsecutionTyping "Strong"^^:esecutionTimeTyping ,
                          "Strong"^^<internal:anonymous-constants> ;
      :hasLogo "http://commons.wikimedia.org/wiki/Special:FilePath/Java%20logo.svg" ;
      :hasTyping "Static"^^<internal:anonymous-constants> ,
                 "Strong"^^<internal:anonymous-constants> ;
      rdfs:comment "An high-level, class-based, object-oriented programming language that is designed to have as few implementation dependencies as possible."@en ;
      rdfs:label "Java"@en .


###  http://www.semanticweb.org/patric/ontologies/2025/3/Programming_Languages_Ontology#JavaScript
:JavaScript rdf:type owl:NamedIndividual ,
                     :DeclarativeLanguage ,
                     :FunctionalLanguage ,
                     :HighLevelLanguage ,
                     :ImperativeLanguage ,
                     :InterpretedProgrammingLanguage ,
                     :Multiparadigms ,
                     :ObjectOrientedLanguage ,
                     :ProgrammingLanguage ;
            <http://www.ontologydesignpatterns.org/cp/owl/collectionentity.owl#isMemberOf> :MongoDBLanguageSet ,
                                                                                           :PyCharmLanguageSet ,
                                                                                           :VSCodeLanguageSet ;
            :implements :DeclarativeParadigm ,
                        :EventOrientedParadigm ,
                        :FunctionalParadigm ,
                        :ImperativeParadigm ,
                        :ObjectOrientedParadigm ;
            :originatesFrom :ECMAScript ;
            :use :V8 ;
            :hasCompileTyping "Dynamic" ;
            :hasEsecutionTyping "Weak" ;
            :hasLogo "http://commons.wikimedia.org/wiki/Special:FilePath/Unofficial%20JavaScript%20logo%202.svg" ;
            :hasTyping "Dynamic" ,
                       "Weak" ;
            rdfs:comment "A lightweight, interpreted scripting language commonly used for dynamic content in web development."@en ;
            rdfs:label "JavaScript"@en .


###  http://www.semanticweb.org/patric/ontologies/2025/3/Programming_Languages_Ontology#Javac
:Javac rdf:type owl:NamedIndividual ,
                :Compiler ,
                :HighLevelCompiler ;
       :partOf :JRE ;
       :translateFrom :Java ;
       rdfs:comment "java compiler"@en ;
       rdfs:label "Javac"@en .


###  http://www.semanticweb.org/patric/ontologies/2025/3/Programming_Languages_Ontology#Jeff_Bezanson
:Jeff_Bezanson rdf:type owl:NamedIndividual ,
                        :ProgrammingLanguageCreator ,
                        <http://xmlns.com/foaf/0.1/Agent> ;
               :isCreatorOf :Julia ;
               rdfs:comment "Creator of Programming Language"@en ;
               rdfs:label "Jeff Bezanson"@en .


###  http://www.semanticweb.org/patric/ontologies/2025/3/Programming_Languages_Ontology#José_Valim
:José_Valim rdf:type owl:NamedIndividual ,
                     :ProgrammingLanguageCreator ,
                     <http://xmlns.com/foaf/0.1/Agent> ;
            :isCreatorOf :Elixir ;
            rdfs:comment "Creator of Programming Language"@en ;
            rdfs:label "José Valim"@en .


###  http://www.semanticweb.org/patric/ontologies/2025/3/Programming_Languages_Ontology#Julia
:Julia rdf:type owl:NamedIndividual ,
                :CompiledProgrammingLanguage ,
                :DeclarativeLanguage ,
                :FunctionalLanguage ,
                :HighLevelLanguage ,
                :HybridProgrammingLanguage ,
                :ImperativeLanguage ,
                :InterpretedProgrammingLanguage ,
                :Multiparadigms ,
                :ObjectOrientedLanguage ,
                :ProgrammingLanguage ,
                :SemiCompiledProgrammingLanguage ;
       :createdBy :Jeff_Bezanson ;
       :implements :DeclarativeParadigm ,
                   :FunctionalParadigm ,
                   :ImperativeParadigm ,
                   :ObjectOrientedParadigm ;
       :originatesFrom :Lisp ;
       :use :JuliaC ,
            :Julia_Runtime ;
       :hasCompileTyping "Dynamic" ;
       :hasEsecutionTyping "Strong" ;
       :hasLogo "http://commons.wikimedia.org/wiki/Special:FilePath/Julia%20logo.svg" ;
       :hasTyping "Dynamic" ,
                  "Strong" ;
       rdfs:comment "A high-level, high-performance programming language for technical computing, with syntax similar to Python and MATLAB."@en ;
       rdfs:label "Julia"@en .


###  http://www.semanticweb.org/patric/ontologies/2025/3/Programming_Languages_Ontology#JuliaC
:JuliaC rdf:type owl:NamedIndividual ,
                 :Compiler ,
                 :HighLevelCompiler ;
        :translateFrom :Julia ;
        rdfs:comment "compiler for the Julia programming language"@en ;
        rdfs:label "JuliaC"@en .


###  http://www.semanticweb.org/patric/ontologies/2025/3/Programming_Languages_Ontology#Julia_Runtime
:Julia_Runtime rdf:type owl:NamedIndividual ,
                        :Interpreter ;
               :executionRowByRowFrom :Julia ;
               rdfs:comment "Interpreter of some Programming Language"@en ;
               rdfs:label "Julia Runtime"@en .


###  http://www.semanticweb.org/patric/ontologies/2025/3/Programming_Languages_Ontology#Kotlin
:Kotlin rdf:type owl:NamedIndividual ,
                 :CompiledProgrammingLanguage ,
                 :HighLevelLanguage ,
                 :HybridProgrammingLanguage ,
                 :ImperativeLanguage ,
                 :InterpretedProgrammingLanguage ,
                 :Multiparadigms ,
                 :ObjectOrientedLanguage ,
                 :ProgrammingLanguage ;
        <http://www.ontologydesignpatterns.org/cp/owl/collectionentity.owl#isMemberOf> :IntellijLanguageSet ;
        :IndirecltyDerivationFrom <http://www.semanticweb.org/patric/ontologies/2025/3/Programming_Languages_Ontology#C++> ;
        :canTranslateInto :x86MachineCode ;
        :implements :ImperativeParadigm ,
                    :ObjectOrientedParadigm ;
        :originatesFrom :Java ;
        :use :JVM ,
             :Kotlinc ;
        :hasCompileTyping "Static"^^:compileTimeTyping ,
                          "Static"^^<internal:anonymous-constants> ;
        :hasEsecutionTyping "Strong"^^:compileTimeTyping ,
                            "Strong"^^<internal:anonymous-constants> ;
        :hasTyping "Static"^^<internal:anonymous-constants> ,
                   "Strong"^^<internal:anonymous-constants> ;
        rdfs:comment "A modern, statically typed programming language that runs on the Java Virtual Machine (JVM) and is fully interoperable with Java"@en ;
        rdfs:label "Kotlin"@en .


###  http://www.semanticweb.org/patric/ontologies/2025/3/Programming_Languages_Ontology#Kotlinc
:Kotlinc rdf:type owl:NamedIndividual ,
                  :Compiler ,
                  :HighLevelCompiler ;
         :translateFrom :Kotlin ;
         :translatesInto :x86MachineCode ;
         :compatibleWith "cross-platform"^^:architectureType ,
                         "cross-platform"^^<internal:anonymous-constants> ;
         rdfs:comment "Kotlin Compiler"@en ;
         rdfs:label "Kotlinc"@en .


###  http://www.semanticweb.org/patric/ontologies/2025/3/Programming_Languages_Ontology#Kubernetes
:Kubernetes rdf:type owl:NamedIndividual ,
                     <http://schema.org/SoftwareApplication> ;
            :writeIn :KubernetesLanguageSet ;
            rdfs:comment "An open-source platform for automating deployment, scaling, and management of containerized applications"@en ;
            rdfs:label "Kubernetes"@en .


###  http://www.semanticweb.org/patric/ontologies/2025/3/Programming_Languages_Ontology#KubernetesLanguageSet
:KubernetesLanguageSet rdf:type owl:NamedIndividual ,
                                <http://www.ontologydesignpatterns.org/cp/owl/collectionentity.owl#Collection> ,
                                <http://www.ontologydesignpatterns.org/cp/owl/set.owl#Set> ,
                                :ProgrammingLanguageSet ;
                       <http://www.ontologydesignpatterns.org/cp/owl/collectionentity.owl#hasMember> :GoLang ;
                       rdfs:comment "Set of Programming Languages of Kubernetes"@en ;
                       rdfs:label "KubernetesLanguageSet"@en .


###  http://www.semanticweb.org/patric/ontologies/2025/3/Programming_Languages_Ontology#Larry_Wall
:Larry_Wall rdf:type owl:NamedIndividual ,
                     :ProgrammingLanguageCreator ,
                     <http://xmlns.com/foaf/0.1/Agent> ;
            :isCreatorOf :Perl ;
            rdfs:comment "Creator of Programming Language"@en ;
            rdfs:label "Larry Wall"@en .


###  http://www.semanticweb.org/patric/ontologies/2025/3/Programming_Languages_Ontology#Lisp
:Lisp rdf:type owl:NamedIndividual ,
               :DeclarativeLanguage ,
               :FunctionalLanguage ,
               :ImperativeLanguage ,
               :Multiparadigms ,
               :ProgrammingLanguage ;
      :implements :DeclarativeParadigm ,
                  :FunctionalParadigm ,
                  :ImperativeParadigm ;
      :hasCompileTyping "Dynamic"^^:compileTimeTyping ,
                        "Dynamic"^^<internal:anonymous-constants> ;
      :hasEsecutionTyping "Strong"^^:esecutionTimeTyping ,
                          "Strong"^^<internal:anonymous-constants> ;
      :hasTyping "Dynamic"^^<internal:anonymous-constants> ,
                 "Strong"^^<internal:anonymous-constants> ;
      rdfs:comment "One of the oldest high-level programming languages, known for its fully parenthesized prefix notation and strong support for symbolic computation."@en ;
      rdfs:label "Lisp"@en .


###  http://www.semanticweb.org/patric/ontologies/2025/3/Programming_Languages_Ontology#LogicParadigm
:LogicParadigm rdf:type owl:NamedIndividual ,
                        :ProgrammingParadigm ;
               rdfs:comment "A programming paradigm based on formal logic, where programs consist of a set of logical statements and computation is performed through logical inference."@en ;
               rdfs:label "LogicParadigm"@en .


###  http://www.semanticweb.org/patric/ontologies/2025/3/Programming_Languages_Ontology#Martin_Odersky
:Martin_Odersky rdf:type owl:NamedIndividual ,
                         :ProgrammingLanguageCreator ,
                         <http://xmlns.com/foaf/0.1/Agent> ;
                :isCreatorOf :Scala ;
                rdfs:comment "Creator of Programming Language"@en ;
                rdfs:label "Martin Odersky"@en .


###  http://www.semanticweb.org/patric/ontologies/2025/3/Programming_Languages_Ontology#MicrosoftWord
:MicrosoftWord rdf:type owl:NamedIndividual ,
                        <http://schema.org/SoftwareApplication> ;
               :writeIn :MicrosoftWordLanguageSet ;
               rdfs:comment "A widely used word processing software developed by Microsoft, featuring document creation, editing, formatting, and collaboration tools."@en ;
               rdfs:label "Microsoft Word"@en .


###  http://www.semanticweb.org/patric/ontologies/2025/3/Programming_Languages_Ontology#MicrosoftWordLanguageSet
:MicrosoftWordLanguageSet rdf:type owl:NamedIndividual ,
                                   <http://www.ontologydesignpatterns.org/cp/owl/collectionentity.owl#Collection> ,
                                   <http://www.ontologydesignpatterns.org/cp/owl/set.owl#Set> ,
                                   :ProgrammingLanguageSet ;
                          <http://www.ontologydesignpatterns.org/cp/owl/collectionentity.owl#hasMember> :C ,
                                                                                                        <http://www.semanticweb.org/patric/ontologies/2025/3/Programming_Languages_Ontology#C++> ;
                          rdfs:comment "Set of Programming Languages of Microsoft Word"@en ;
                          rdfs:label "MicrosoftWordLanguageSet"@en .


###  http://www.semanticweb.org/patric/ontologies/2025/3/Programming_Languages_Ontology#MongoDB
:MongoDB rdf:type owl:NamedIndividual ,
                  <http://schema.org/SoftwareApplication> ;
         :writeIn :MongoDBLanguageSet ;
         rdfs:comment "A popular open-source NoSQL database that stores data in flexible, JSON-like documents, designed for scalability and high performance."@en ;
         rdfs:label "MongoDB"@en .


###  http://www.semanticweb.org/patric/ontologies/2025/3/Programming_Languages_Ontology#MongoDBLanguageSet
:MongoDBLanguageSet rdf:type owl:NamedIndividual ,
                             <http://www.ontologydesignpatterns.org/cp/owl/collectionentity.owl#Collection> ,
                             <http://www.ontologydesignpatterns.org/cp/owl/set.owl#Set> ,
                             :ProgrammingLanguageSet ;
                    <http://www.ontologydesignpatterns.org/cp/owl/collectionentity.owl#hasMember> :Java ,
                                                                                                  :JavaScript ;
                    rdfs:comment "Set of Programming Languages for MongoDB."@en ;
                    rdfs:label "MongoDBLanguageSet"@en .


###  http://www.semanticweb.org/patric/ontologies/2025/3/Programming_Languages_Ontology#MySQL
:MySQL rdf:type owl:NamedIndividual ,
                :Compiler ,
                :HighLevelCompiler ;
       :translateFrom :SQL ;
       :compatibleWith "x86-64" ;
       rdfs:comment "SQL database engine software"@en ;
       rdfs:label "MySQL"@en .


###  http://www.semanticweb.org/patric/ontologies/2025/3/Programming_Languages_Ontology#ObjectOrientedParadigm
:ObjectOrientedParadigm rdf:type owl:NamedIndividual ,
                                 :ProgrammingParadigm ;
                        rdfs:comment "A programming paradigm based on the concept of objects, which encapsulate data and behavior, promoting modularity, reuse, and abstraction."@en ;
                        rdfs:label "ObjectOrientedParadigm"@en .


###  http://www.semanticweb.org/patric/ontologies/2025/3/Programming_Languages_Ontology#Objective-C
:Objective-C rdf:type owl:NamedIndividual ,
                      :CompiledProgrammingLanguage ,
                      :HighLevelLanguage ,
                      :ImperativeLanguage ,
                      :Multiparadigms ,
                      :ObjectOrientedLanguage ,
                      :ProceduralLanguage ,
                      :ProgrammingLanguage ;
             :canTranslateInto :x86MachineCode ;
             :implements :ImperativeParadigm ,
                         :ObjectOrientedParadigm ,
                         :ProceduralParadigm ;
             :originatesFrom :C ;
             :use :GCC ;
             :hasCompileTyping "Static"^^:compileTimeTyping ,
                               "Static"^^<internal:anonymous-constants> ;
             :hasEsecutionTyping "Strong"^^:esecutionTimeTyping ,
                                 "Strong"^^<internal:anonymous-constants> ;
             :hasTyping "Static"^^<internal:anonymous-constants> ,
                        "Strong"^^<internal:anonymous-constants> ;
             rdfs:comment "A general-purpose, object-oriented programming language that adds Smalltalk-style messaging to the C programming language, widely used for macOS and iOS development."@en ;
             rdfs:label "Objective-C"@en .


###  http://www.semanticweb.org/patric/ontologies/2025/3/Programming_Languages_Ontology#PHP
:PHP rdf:type owl:NamedIndividual ,
              :CompiledProgrammingLanguage ,
              :HighLevelLanguage ,
              :HybridProgrammingLanguage ,
              :ImperativeLanguage ,
              :InterpretedProgrammingLanguage ,
              :Multiparadigms ,
              :ProceduralLanguage ,
              :ProgrammingLanguage ,
              :SemiCompiledProgrammingLanguage ;
     <http://www.ontologydesignpatterns.org/cp/owl/collectionentity.owl#isMemberOf> :VSCodeLanguageSet ;
     :createdBy :Rasmus_Lerdorf ;
     :implements :ImperativeParadigm ,
                 :ProceduralParadigm ;
     :originatesFrom :C ;
     :use :Zend ,
          :Zend_Engine ;
     :hasCompileTyping "Dynamic" ;
     :hasEsecutionTyping "Weak" ;
     :hasLogo "http://commons.wikimedia.org/wiki/Special:FilePath/PHP%20logo.svg" ;
     :hasTyping "Dynamic" ,
                "Weak" ;
     rdfs:comment "A server-side scripting language designed for web development but also used as a general-purpose programming language."@en ;
     rdfs:label "PHP"@en .


###  http://www.semanticweb.org/patric/ontologies/2025/3/Programming_Languages_Ontology#Perl
:Perl rdf:type owl:NamedIndividual ,
               :DeclarativeLanguage ,
               :FunctionalLanguage ,
               :HighLevelLanguage ,
               :ImperativeLanguage ,
               :InterpretedProgrammingLanguage ,
               :Multiparadigms ,
               :ObjectOrientedLanguage ,
               :ProgrammingLanguage ;
      :createdBy :Larry_Wall ;
      :implements :DeclarativeParadigm ,
                  :FunctionalParadigm ,
                  :ImperativeParadigm ,
                  :ObjectOrientedParadigm ;
      :originatesFrom :C ;
      :use :Perl_Interpreter ;
      :hasCompileTyping "Dynamic" ;
      :hasEsecutionTyping "Weak" ;
      :hasLogo "http://commons.wikimedia.org/wiki/Special:FilePath/Perl%20logo.svg" ;
      :hasTyping "Dynamic" ,
                 "Weak" ;
      rdfs:comment "A high-level, interpreted language known for its text processing capabilities and flexibility in web development."@en ;
      rdfs:label "Perl"@en .


###  http://www.semanticweb.org/patric/ontologies/2025/3/Programming_Languages_Ontology#Perl_Interpreter
:Perl_Interpreter rdf:type owl:NamedIndividual ,
                           :Interpreter ;
                  :executionRowByRowFrom :Perl ;
                  rdfs:comment "Interpreter of some Programming Language"@en ;
                  rdfs:label "Perl Interpreter"@en .


###  http://www.semanticweb.org/patric/ontologies/2025/3/Programming_Languages_Ontology#ProceduralParadigm
:ProceduralParadigm rdf:type owl:NamedIndividual ,
                             :ProgrammingParadigm ;
                    rdfs:comment "A programming paradigm that structures programs as sequences of procedures or routines, emphasizing a step-by-step approach to problem solving."@en ;
                    rdfs:label "ProceduralParadigm"@en .


###  http://www.semanticweb.org/patric/ontologies/2025/3/Programming_Languages_Ontology#Protegè
:Protegè rdf:type owl:NamedIndividual ,
                  <http://schema.org/SoftwareApplication> ;
         :writeIn :ProtègèLanguageSet ;
         rdfs:comment "An open-source ontology editor and knowledge management system used for creating, visualizing, and managing ontologies."@en ;
         rdfs:label "Protégé"@en .


###  http://www.semanticweb.org/patric/ontologies/2025/3/Programming_Languages_Ontology#ProtègèLanguageSet
:ProtègèLanguageSet rdf:type owl:NamedIndividual ,
                             <http://www.ontologydesignpatterns.org/cp/owl/collectionentity.owl#Collection> ,
                             <http://www.ontologydesignpatterns.org/cp/owl/set.owl#Set> ,
                             :ProgrammingLanguageSet ;
                    <http://www.ontologydesignpatterns.org/cp/owl/collectionentity.owl#hasMember> :Java ;
                    rdfs:comment "Protégé's Programming Languages Set"@en ;
                    rdfs:label "ProtègèLanguageSet"@en .


###  http://www.semanticweb.org/patric/ontologies/2025/3/Programming_Languages_Ontology#PyCharm
:PyCharm rdf:type owl:NamedIndividual ,
                  :DevelopmentEnvironment ;
         :allowsDevelopmentOf :PyCharmLanguageSet ;
         rdfs:comment "An integrated development environment (IDE) developed by JetBrains, designed specifically for Python programming with features like intelligent code completion, debugging, and testing."@en ;
         rdfs:label "PyCharm"@en .


###  http://www.semanticweb.org/patric/ontologies/2025/3/Programming_Languages_Ontology#PyCharmLanguageSet
:PyCharmLanguageSet rdf:type owl:NamedIndividual ,
                             <http://www.ontologydesignpatterns.org/cp/owl/collectionentity.owl#Collection> ,
                             <http://www.ontologydesignpatterns.org/cp/owl/set.owl#Set> ,
                             :ProgrammingLanguageSet ;
                    <http://www.ontologydesignpatterns.org/cp/owl/collectionentity.owl#hasMember> :JavaScript ,
                                                                                                  :Python ,
                                                                                                  :SQL ;
                    rdfs:comment "Supported PyCharm Language Set"@en ;
                    rdfs:label "PyCharmLanguageSet"@en .


###  http://www.semanticweb.org/patric/ontologies/2025/3/Programming_Languages_Ontology#Python
:Python rdf:type owl:NamedIndividual ,
                 :CompiledProgrammingLanguage ,
                 :DeclarativeLanguage ,
                 :FunctionalLanguage ,
                 :HighLevelLanguage ,
                 :HybridProgrammingLanguage ,
                 :ImperativeLanguage ,
                 :InterpretedProgrammingLanguage ,
                 :Multiparadigms ,
                 :ObjectOrientedLanguage ,
                 :ProceduralLanguage ,
                 :ProgrammingLanguage ,
                 :SemiCompiledProgrammingLanguage ;
        <http://www.ontologydesignpatterns.org/cp/owl/collectionentity.owl#isMemberOf> :PyCharmLanguageSet ,
                                                                                       :VSCodeLanguageSet ;
        :createdBy :Guido_van_Rossum ;
        :implements :DeclarativeParadigm ,
                    :FunctionalParadigm ,
                    :ImperativeParadigm ,
                    :ObjectOrientedParadigm ,
                    :ProceduralParadigm ;
        :originatesFrom :ABC ;
        :use :CPython ;
        :hasCompileTyping "Dynamic" ;
        :hasEsecutionTyping "Strong" ;
        :hasTyping "Dynamic" ,
                   "Strong" ;
        rdfs:comment "A high-level, interpreted programming language known for its readability and broad applicability in web development, data science, AI, and more."@en ;
        rdfs:label "Python"@en .


###  http://www.semanticweb.org/patric/ontologies/2025/3/Programming_Languages_Ontology#Rasmus_Lerdorf
:Rasmus_Lerdorf rdf:type owl:NamedIndividual ,
                         :ProgrammingLanguageCreator ,
                         <http://xmlns.com/foaf/0.1/Agent> ;
                :isCreatorOf :PHP ;
                rdfs:comment "Creator of Programming Language"@en ;
                rdfs:label "Rasmus Lerdorf"@en .


###  http://www.semanticweb.org/patric/ontologies/2025/3/Programming_Languages_Ontology#Robert_Griesemer
:Robert_Griesemer rdf:type owl:NamedIndividual ,
                           :ProgrammingLanguageCreator ,
                           <http://xmlns.com/foaf/0.1/Agent> ;
                  :isCreatorOf :GoLang ;
                  rdfs:comment "Creator of Programming Language"@en ;
                  rdfs:label "Robert Griesemer"@en .


###  http://www.semanticweb.org/patric/ontologies/2025/3/Programming_Languages_Ontology#Rust
:Rust rdf:type owl:NamedIndividual ,
               :CompiledProgrammingLanguage ,
               :HighLevelLanguage ,
               :ImperativeLanguage ,
               :Multiparadigms ,
               :ProceduralLanguage ,
               :ProgrammingLanguage ;
      <http://www.ontologydesignpatterns.org/cp/owl/collectionentity.owl#isMemberOf> :VSCodeLanguageSet ;
      :IndirecltyDerivationFrom :C ;
      :canTranslateInto :x86MachineCode ;
      :createdBy :Graydon_Hoare ;
      :implements :ImperativeParadigm ,
                  :ProceduralParadigm ;
      :originatesFrom <http://www.semanticweb.org/patric/ontologies/2025/3/Programming_Languages_Ontology#C++> ;
      :use :Rustc ;
      :hasCompileTyping "Static" ;
      :hasEsecutionTyping "Strong" ;
      :hasLogo "http://commons.wikimedia.org/wiki/Special:FilePath/Rust%20logo%20black.svg" ;
      :hasTyping "Static" ,
                 "Strong" ;
      rdfs:comment "A systems programming language focused on safety and concurrency, known for its memory safety guarantees without a garbage collector."@en ;
      rdfs:label "Rust"@en .


###  http://www.semanticweb.org/patric/ontologies/2025/3/Programming_Languages_Ontology#Rustc
:Rustc rdf:type owl:NamedIndividual ,
                :Compiler ,
                :HighLevelCompiler ;
       :translateFrom :Rust ;
       :translatesInto :x86MachineCode ;
       :compatibleWith "cross-platform" ;
       rdfs:comment "compiler of the Rust programming language"@en ;
       rdfs:label "Rustc"@en .


###  http://www.semanticweb.org/patric/ontologies/2025/3/Programming_Languages_Ontology#SQL
:SQL rdf:type owl:NamedIndividual ,
              :CompiledProgrammingLanguage ,
              :HighLevelLanguage ,
              :HybridProgrammingLanguage ,
              :ImperativeLanguage ,
              :InterpretedProgrammingLanguage ,
              :Multiparadigms ,
              :ProgrammingLanguage ,
              :StructuralLanguage ;
     <http://www.ontologydesignpatterns.org/cp/owl/collectionentity.owl#isMemberOf> :PyCharmLanguageSet ;
     :createdBy :Donald_D._Chamberlin ;
     :implements :ImperativeParadigm ,
                 :StructuralParadigm ;
     :use :Database_Engine ,
          :MySQL ;
     :hasCompileTyping "Dynamic" ;
     :hasEsecutionTyping "Weak" ;
     :hasLogo "http://commons.wikimedia.org/wiki/Special:FilePath/SQL%20logo.svg" ;
     :hasTyping "Dynamic" ,
                "Weak" ;
     rdfs:comment "A domain-specific language used in programming and managing relational databases, known for its declarative syntax."@en ;
     rdfs:label "SQL"@en .


###  http://www.semanticweb.org/patric/ontologies/2025/3/Programming_Languages_Ontology#Scala
:Scala rdf:type owl:NamedIndividual ,
                :CompiledProgrammingLanguage ,
                :DeclarativeLanguage ,
                :FunctionalLanguage ,
                :HighLevelLanguage ,
                :HybridProgrammingLanguage ,
                :ImperativeLanguage ,
                :InterpretedProgrammingLanguage ,
                :Multiparadigms ,
                :ObjectOrientedLanguage ,
                :ProgrammingLanguage ,
                :SemiCompiledProgrammingLanguage ;
       :IndirecltyDerivationFrom <http://www.semanticweb.org/patric/ontologies/2025/3/Programming_Languages_Ontology#C++> ;
       :createdBy :Martin_Odersky ;
       :implements :DeclarativeParadigm ,
                   :EventOrientedParadigm ,
                   :FunctionalParadigm ,
                   :ImperativeParadigm ,
                   :ObjectOrientedParadigm ;
       :originatesFrom :Java ;
       :use :JVM ,
            :Scalac ;
       :hasCompileTyping "Static" ;
       :hasEsecutionTyping "Strong" ;
       :hasLogo "http://commons.wikimedia.org/wiki/Special:FilePath/Scala%20logo.svg" ;
       :hasTyping "Static" ,
                  "Strong" ;
       rdfs:comment "A hybrid functional and object-oriented programming language that runs on the Java Virtual Machine (JVM)."@en ;
       rdfs:label "Scala"@en .


###  http://www.semanticweb.org/patric/ontologies/2025/3/Programming_Languages_Ontology#Scalac
:Scalac rdf:type owl:NamedIndividual ,
                 :Compiler ,
                 :HighLevelCompiler ;
        :translateFrom :Scala ;
        rdfs:comment "compiler for the Scala programming language"@en ;
        rdfs:label "Scalac"@en .


###  http://www.semanticweb.org/patric/ontologies/2025/3/Programming_Languages_Ontology#StructuralParadigm
:StructuralParadigm rdf:type owl:NamedIndividual ,
                             :ProgrammingParadigm ;
                    rdfs:comment "A programming paradigm focused on the organization and structure of code, often emphasizing modularity and clear control flow through structures like loops and conditionals."@en ;
                    rdfs:label "StructuralParadigm"@en .


###  http://www.semanticweb.org/patric/ontologies/2025/3/Programming_Languages_Ontology#Swift
:Swift rdf:type owl:NamedIndividual ,
                :CompiledProgrammingLanguage ,
                :HighLevelLanguage ,
                :ImperativeLanguage ,
                :Multiparadigms ,
                :ProceduralLanguage ,
                :ProgrammingLanguage ;
       :IndirecltyDerivationFrom :C ;
       :canTranslateInto :x86MachineCode ;
       :createdBy :Chris_Lattner ;
       :implements :ImperativeParadigm ,
                   :ProceduralParadigm ;
       :originatesFrom :Objective-C ;
       :use :Swiftc ;
       :hasCompileTyping "Static" ;
       :hasEsecutionTyping "Strong" ;
       :hasLogo "http://commons.wikimedia.org/wiki/Special:FilePath/Swift%20logo.svg" ;
       :hasTyping "Static" ,
                  "Strong" ;
       rdfs:comment "A modern programming language developed by Apple for iOS and macOS development, known for its safety and performance."@en ;
       rdfs:label "Swift"@en .


###  http://www.semanticweb.org/patric/ontologies/2025/3/Programming_Languages_Ontology#SwiftUI
:SwiftUI rdf:type owl:NamedIndividual ,
                  :CompiledProgrammingLanguage ,
                  :HighLevelLanguage ,
                  :ImperativeLanguage ,
                  :Multiparadigms ,
                  :ProceduralLanguage ,
                  :ProgrammingLanguage ;
         :IndirecltyDerivationFrom :C ;
         :createdBy :Chris_Lattner ;
         :implements :ImperativeParadigm ,
                     :ProceduralParadigm ;
         :originatesFrom :Objective-C ;
         :use :SwiftUIC ;
         :hasCompileTyping "Static" ;
         :hasEsecutionTyping "Strong" ;
         :hasLogo "http://commons.wikimedia.org/wiki/Special:FilePath/SwiftUI%20logo.svg" ;
         :hasTyping "Static" ,
                    "Strong" ;
         rdfs:comment "A declarative framework for building user interfaces across all Apple platforms, using Swift."@en ;
         rdfs:label "SwiftUI"@en .


###  http://www.semanticweb.org/patric/ontologies/2025/3/Programming_Languages_Ontology#SwiftUIC
:SwiftUIC rdf:type owl:NamedIndividual ,
                   :Compiler ,
                   :HighLevelCompiler ;
          :translateFrom :SwiftUI .


###  http://www.semanticweb.org/patric/ontologies/2025/3/Programming_Languages_Ontology#Swiftc
:Swiftc rdf:type owl:NamedIndividual ,
                 :Compiler ,
                 :HighLevelCompiler ;
        :translateFrom :Swift ;
        :translatesInto :x86MachineCode ;
        :compatibleWith "cross-platform"^^:architectureType ,
                        "cross-platform"^^<internal:anonymous-constants> ;
        rdfs:comment "compiler of the Swift programming language"@en ;
        rdfs:label "Swiftc"@en .


###  http://www.semanticweb.org/patric/ontologies/2025/3/Programming_Languages_Ontology#TSC
:TSC rdf:type owl:NamedIndividual ,
              :Compiler ,
              :HighLevelCompiler ;
     :translateFrom :TypeScript ;
     :compatibleWith "Node.js" ;
     rdfs:comment "compiler of TypeScript in Javascript"@en ;
     rdfs:label "TSC"@en .


###  http://www.semanticweb.org/patric/ontologies/2025/3/Programming_Languages_Ontology#TypeScript
:TypeScript rdf:type owl:NamedIndividual ,
                     :CompiledProgrammingLanguage ,
                     :DeclarativeLanguage ,
                     :FunctionalLanguage ,
                     :HighLevelLanguage ,
                     :HybridProgrammingLanguage ,
                     :ImperativeLanguage ,
                     :InterpretedProgrammingLanguage ,
                     :Multiparadigms ,
                     :ObjectOrientedLanguage ,
                     :ProgrammingLanguage ,
                     :SemiCompiledProgrammingLanguage ;
            <http://www.ontologydesignpatterns.org/cp/owl/collectionentity.owl#isMemberOf> :VSCodeLanguageSet ;
            :IndirecltyDerivationFrom :ECMAScript ;
            :createdBy :Anders_Hejlsberg ;
            :implements :DeclarativeParadigm ,
                        :EventOrientedParadigm ,
                        :FunctionalParadigm ,
                        :ImperativeParadigm ,
                        :ObjectOrientedParadigm ;
            :originatesFrom :JavaScript ;
            :use :TSC ,
                 :V8 ;
            :hasCompileTyping "Static" ;
            :hasEsecutionTyping "Strong" ;
            :hasLogo "http://commons.wikimedia.org/wiki/Special:FilePath/TypeScript%20logo.svg" ;
            :hasTyping "Static" ,
                       "Strong" ;
            rdfs:comment "A superset of JavaScript that adds static typing and is designed for large-scale application development."@en ;
            rdfs:label "TypeScript"@en .


###  http://www.semanticweb.org/patric/ontologies/2025/3/Programming_Languages_Ontology#V8
:V8 rdf:type owl:NamedIndividual ,
             :Interpreter ;
    :executionRowByRowFrom :ECMAScript ,
                           :JavaScript ,
                           :TypeScript ;
    rdfs:comment "Interpreter of some Programming Language"@en ;
    rdfs:label "V8"@en .


###  http://www.semanticweb.org/patric/ontologies/2025/3/Programming_Languages_Ontology#VBC
:VBC rdf:type owl:NamedIndividual ,
              :Compiler ,
              :HighLevelCompiler ;
     :translateFrom :Visual_Basic ;
     rdfs:comment "compiler for the Visual Basic .NET programming language"@en ;
     rdfs:label "VBC"@en .


###  http://www.semanticweb.org/patric/ontologies/2025/3/Programming_Languages_Ontology#VSCodeLanguageSet
:VSCodeLanguageSet rdf:type owl:NamedIndividual ,
                            <http://www.ontologydesignpatterns.org/cp/owl/collectionentity.owl#Collection> ,
                            <http://www.ontologydesignpatterns.org/cp/owl/set.owl#Set> ,
                            :ProgrammingLanguageSet ;
                   <http://www.ontologydesignpatterns.org/cp/owl/collectionentity.owl#hasMember> :C ,
                                                                                                 :Java ,
                                                                                                 :JavaScript ,
                                                                                                 :PHP ,
                                                                                                 :Python ,
                                                                                                 :Rust ,
                                                                                                 :TypeScript ,
                                                                                                 <http://www.semanticweb.org/patric/ontologies/2025/3/Programming_Languages_Ontology#C++> ;
                   rdfs:comment "Programming Languages supported by Visual Studio Code"@en ;
                   rdfs:label "VSCodeLanguageSet"@en .


###  http://www.semanticweb.org/patric/ontologies/2025/3/Programming_Languages_Ontology#VisualStudioCode
:VisualStudioCode rdf:type owl:NamedIndividual ,
                           :DevelopmentEnvironment ;
                  :allowsDevelopmentOf :VSCodeLanguageSet ;
                  rdfs:comment "A lightweight, open-source code editor developed by Microsoft, featuring support for multiple programming languages, extensions, debugging, and version control integration."@en ;
                  rdfs:label "VisualStudioCode"@en .


###  http://www.semanticweb.org/patric/ontologies/2025/3/Programming_Languages_Ontology#Visual_Basic
:Visual_Basic rdf:type owl:NamedIndividual ,
                       :CompiledProgrammingLanguage ,
                       :HighLevelLanguage ,
                       :HybridProgrammingLanguage ,
                       :ImperativeLanguage ,
                       :InterpretedProgrammingLanguage ,
                       :Multiparadigms ,
                       :ProceduralLanguage ,
                       :ProgrammingLanguage ,
                       :SemiCompiledProgrammingLanguage ;
              :createdBy :Alan_Cooper ;
              :implements :ImperativeParadigm ,
                          :ProceduralParadigm ;
              :use :VBC ;
              :hasCompileTyping "Static" ;
              :hasEsecutionTyping "Weak" ;
              :hasLogo "http://commons.wikimedia.org/wiki/Special:FilePath/Visual%20Basic%20logo.svg" ;
              :hasTyping "Static" ,
                         "Weak" ;
              rdfs:comment "An event-driven programming language from Microsoft known for its ease of use in developing Windows applications."@en ;
              rdfs:label "Visual Basic"@en .


###  http://www.semanticweb.org/patric/ontologies/2025/3/Programming_Languages_Ontology#Zend
:Zend rdf:type owl:NamedIndividual ,
               :Compiler ,
               :HighLevelCompiler ;
      :translateFrom :PHP ;
      :compatibleWith "cross-platform" ;
      rdfs:comment "open source scripting engine that can be used to interpret the PHP programming language"@en ;
      rdfs:label "Zend"@en .


###  http://www.semanticweb.org/patric/ontologies/2025/3/Programming_Languages_Ontology#Zend_Engine
:Zend_Engine rdf:type owl:NamedIndividual ,
                      :Interpreter ;
             :executionRowByRowFrom :PHP ;
             rdfs:comment "Interpreter of some Programming Language"@en ;
             rdfs:label "Zend Engine"@en .


###  http://www.semanticweb.org/patric/ontologies/2025/3/Programming_Languages_Ontology#x86MachineCode
:x86MachineCode rdf:type owl:NamedIndividual ,
                         :LowLevelLanguage ,
                         :MachineLanguage ,
                         :ProgrammingLanguage ;
                :translatableBy :CrystalC ,
                                :GCC ,
                                :Kotlinc ,
                                :Rustc ,
                                :Swiftc ;
                :executableBy "AMD"^^:architectureType ,
                              "AMD"^^<internal:anonymous-constants> ,
                              "INTEL"^^:architectureType ,
                              "INTEL"^^<internal:anonymous-constants> ;
                rdfs:comment "The low-level binary instructions executed directly by x86 processors, representing the fundamental commands understood by the hardware."@en ;
                rdfs:label "x86MachineCode"@en .


###  http://www.semanticweb.org/patric/ontologies/2025/3/Programming_Languages_Ontology#C++
<http://www.semanticweb.org/patric/ontologies/2025/3/Programming_Languages_Ontology#C++> rdf:type owl:NamedIndividual ,
                                                                                                  :CompiledProgrammingLanguage ,
                                                                                                  :HighLevelLanguage ,
                                                                                                  :ImperativeLanguage ,
                                                                                                  :Multiparadigms ,
                                                                                                  :ProceduralLanguage ,
                                                                                                  :ProgrammingLanguage ,
                                                                                                  :StructuralLanguage ;
                                                                                         <http://www.ontologydesignpatterns.org/cp/owl/collectionentity.owl#isMemberOf> :MicrosoftWordLanguageSet ,
                                                                                                                                                                        :VSCodeLanguageSet ;
                                                                                         :canTranslateInto :x86MachineCode ;
                                                                                         :createdBy :Bjarne_Stroustrup ;
                                                                                         :implements :ImperativeParadigm ,
                                                                                                     :ProceduralParadigm ,
                                                                                                     :StructuralParadigm ;
                                                                                         :originatesFrom :C ;
                                                                                         :use :GCC ;
                                                                                         :hasCompileTyping "Static" ;
                                                                                         :hasEsecutionTyping "Strong" ;
                                                                                         :hasLogo "http://commons.wikimedia.org/wiki/Special:FilePath/C%2B%2B%20logo.svg" ;
                                                                                         :hasTyping "Static" ,
                                                                                                    "Strong" ;
                                                                                         rdfs:comment "An extension of the C programming language that includes object-oriented features, widely used for system and application software development."@en ;
                                                                                         rdfs:label "C++"@en .


#################################################################
#    Annotations
#################################################################

<http://www.ontologydesignpatterns.org/schemas/cpannotationschema.owl#hasComponent> rdfs:comment "This annotation property is useful for content ontology design patterns. Its value is a URI, which refers to another content ontology design pattern which is a component of the annotated one." .


<http://www.ontologydesignpatterns.org/schemas/cpannotationschema.owl#hasUnitTest> rdfs:comment "This property can be used to annotate a unit test (e.g. in the form of a SPARQL query) to be launched to evaluate an ontology against a requirement-based task." .


<http://www.ontologydesignpatterns.org/schemas/cpannotationschema.owl#isCloneOf> rdfs:comment "This annotation property is used for referring a cloned ontology entity to its cloning source." .


<http://www.ontologydesignpatterns.org/schemas/cpannotationschema.owl#isSpecializationOf> rdfs:comment "This annotation property is useful for content ontology design patterns and its elements. Its value is a URI, which refers either to a content ontology design pattern that is specialized by the annotated one, or to an ontology element that is specialized by the annotated one." .


#################################################################
#    General axioms
#################################################################

[ rdf:type owl:AllDifferent ;
  owl:distinctMembers ( :ABC
                        :ABCInterpreter
                        :Alan_Cooper
                        :Anders_Hejlsberg
                        :Ary_Borenszweig
                        :Assembler
                        :Assembly
                        :BEAM_VM
                        :Bjarne_Stroustrup
                        :BrendanEich
                        :C
                        :CPython
                        :Chris_Lattner
                        :Crystal
                        :CrystalC
                        :Database_Engine
                        :DeclarativeParadigm
                        :Dennis_Ritchie
                        :Donald_D._Chamberlin
                        :Dr._Sarah_Nilsson
                        :ECMAScript
                        :Elixir
                        :ElixirC
                        :Erlang
                        :EventOrientedParadigm
                        :FunctionalParadigm
                        :GCC
                        :GoLang
                        :Graydon_Hoare
                        :Guido_van_Rossum
                        :ImperativeParadigm
                        :IntellijIDEA
                        :IntellijLanguageSet
                        :JRE
                        :JVM
                        :James_Gosling
                        :Java
                        :JavaScript
                        :Javac
                        :Jeff_Bezanson
                        :José_Valim
                        :Julia
                        :JuliaC
                        :Julia_Runtime
                        :Kotlin
                        :Kotlinc
                        :Kubernetes
                        :KubernetesLanguageSet
                        :Larry_Wall
                        :Lisp
                        :LogicParadigm
                        :Martin_Odersky
                        :MicrosoftWord
                        :MicrosoftWordLanguageSet
                        :MongoDB
                        :MongoDBLanguageSet
                        :MySQL
                        :ObjectOrientedParadigm
                        :Objective-C
                        :PHP
                        :Perl
                        :Perl_Interpreter
                        :ProceduralParadigm
                        :Protegè
                        :ProtègèLanguageSet
                        :PyCharm
                        :PyCharmLanguageSet
                        :Python
                        :Rasmus_Lerdorf
                        :Robert_Griesemer
                        :Rust
                        :Rustc
                        :SQL
                        :Scala
                        :Scalac
                        :StructuralParadigm
                        :Swift
                        :SwiftUI
                        :SwiftUIC
                        :Swiftc
                        :TSC
                        :TypeScript
                        :V8
                        :VBC
                        :VSCodeLanguageSet
                        :VisualStudioCode
                        :Visual_Basic
                        :Zend
                        :Zend_Engine
                        :x86MachineCode
                        <http://www.semanticweb.org/patric/ontologies/2025/3/Programming_Languages_Ontology#C++>
                      )
] .


[ rdf:type owl:AllDifferent ;
  owl:distinctMembers ( :ABC
                        :C
                        :Crystal
                        :ECMAScript
                        :Elixir
                        :Erlang
                        :GoLang
                        :Java
                        :JavaScript
                        :Julia
                        :Kotlin
                        :Lisp
                        :Objective-C
                        :PHP
                        :Perl
                        :Python
                        :Rust
                        :SQL
                        :Scala
                        :Swift
                        :SwiftUI
                        :TypeScript
                        :Visual_Basic
                        <http://www.semanticweb.org/patric/ontologies/2025/3/Programming_Languages_Ontology#C++>
                      )
] .


[ rdf:type owl:AllDifferent ;
  owl:distinctMembers ( :ABCInterpreter
                        :CPython
                        :Database_Engine
                        :JVM
                        :Julia_Runtime
                        :Perl_Interpreter
                        :V8
                        :Zend_Engine
                      )
] .


[ rdf:type owl:AllDifferent ;
  owl:distinctMembers ( :Alan_Cooper
                        :Anders_Hejlsberg
                        :Ary_Borenszweig
                        :Bjarne_Stroustrup
                        :BrendanEich
                        :Chris_Lattner
                        :Dennis_Ritchie
                        :Donald_D._Chamberlin
                        :Dr._Sarah_Nilsson
                        :Graydon_Hoare
                        :Guido_van_Rossum
                        :James_Gosling
                        :Jeff_Bezanson
                        :José_Valim
                        :Larry_Wall
                        :Martin_Odersky
                        :Rasmus_Lerdorf
                        :Robert_Griesemer
                      )
] .


[ rdf:type owl:AllDifferent ;
  owl:distinctMembers ( :Assembler
                      )
] .


[ rdf:type owl:AllDifferent ;
  owl:distinctMembers ( :Assembly
                        :Java
                      )
] .


[ rdf:type owl:AllDifferent ;
  owl:distinctMembers ( :CrystalC
                        :ElixirC
                        :GCC
                        :Javac
                        :JuliaC
                        :Kotlinc
                        :MySQL
                        :Rustc
                        :Scalac
                        :SwiftUIC
                        :Swiftc
                        :TSC
                        :VBC
                        :Zend
                      )
] .


[ rdf:type owl:AllDifferent ;
  owl:distinctMembers ( :DeclarativeParadigm
                        :EventOrientedParadigm
                        :FunctionalParadigm
                        :ImperativeParadigm
                        :LogicParadigm
                        :ObjectOrientedParadigm
                        :ProceduralParadigm
                        :StructuralParadigm
                      )
] .


[ rdf:type owl:AllDifferent ;
  owl:distinctMembers ( :IntellijIDEA
                        :PyCharm
                        :VisualStudioCode
                      )
] .


[ rdf:type owl:AllDifferent ;
  owl:distinctMembers ( :Kubernetes
                        :MicrosoftWord
                        :MongoDB
                        :Protegè
                      )
] .


###  Generated by the OWL API (version 4.5.9.2019-02-01T07:24:44Z) https://github.com/owlcs/owlapi
